templates/multicopy/general_multicopy.v
@@ -111,7 +111,7 @@ Section multicopy.
   Context {Σ} `{!heapG Σ, !multicopyG Σ}.
   Context (N : namespace).
   Notation iProp := (iProp Σ).
-  Local Notation "m !1 i" := (nzmap_total_lookup i m) (at level 20).
+(*  Local Notation "m !1 i" := (nzmap_total_lookup i m) (at level 20).*)
 
   (** Definitions **)
 
@@ -124,6 +124,11 @@ Section multicopy.
   Hypothesis node_sep_star: ∀ r n es C es' C',
     node r n es C ∗ node r n es' C' -∗ False.
 
+  Hypothesis node_edgeset_disjoint: ∀ r n es C,
+    node r n es C -∗ ⌜∀ n1 n2, n1 ≠ n2 → es !!! n1 ∩ es !!! n2 = ∅⌝.  
+
+  Hypothesis node_edgeset_self_empty: ∀ r n es C,
+    node r n es C -∗ ⌜es !!! n = ∅⌝.
 
   Definition out_edgeset_list (k: K) (esl : list (Node * gset K)) :=             
     list_find (λ ns, k ∈ ns.2) esl.
@@ -170,46 +175,54 @@ Section multicopy.
 
   Definition closed γ_f (es: esT) : iProp := ∀ n, ⌜es !!! n  ≠ ∅⌝ → inFP γ_f n.
 
-  Definition inflow_zero (I: KT_flowint_ur K) : iProp := ⌜∀ n, inset_KT I n = ∅⌝. 
+  Definition inflow_zero (I: KT_flowint_ur K) := ∀ n, inset_KT I n = ∅. 
 
-  Definition inflow_R (R: inset_flowint_ur K) r : iProp := 
-    ⌜∀ n k, if n =? r then in_inset K k R n else ¬ in_inset K k R n⌝. 
+  Definition inflow_R (R: inset_flowint_ur K) r := 
+    ∀ n k, if n =? r then in_inset K k R n else ¬ in_inset K k R n. 
 
   Definition outflow_constraint_I (In: KT_flowint_ur K) (es: esT) 
-                          (Cn Bn: gmap K natUR) : iProp := 
-    ⌜∀ n' k t, (k,t) ∈ outset_KT In n' ↔ 
-                          k ∈ es !!! n' ∧ (Cn !!! k = 0) ∧ (Bn !!! k = t)⌝.
+                          (Cn Bn: gmap K natUR) := 
+    ∀ n' k t, (k,t) ∈ outset_KT In n' ↔ 
+                          k ∈ es !!! n' ∧ (Cn !!! k = 0) ∧ (Bn !!! k = t).
 
   Definition outflow_constraint_J (Jn: KT_flowint_ur K) (es: esT) 
-                          (Cn Bn: gmap K natUR) : iProp := 
-    ⌜∀ n' k t, (k,t) ∈ outset_KT Jn n' ↔ 
-                          k ∈ es !!! n' ∧ (Cn !!! k = t)⌝.
+                          (Cn Bn: gmap K natUR) := 
+    ∀ n' k t, (k,t) ∈ outset_KT Jn n' ↔ 
+                          k ∈ es !!! n' ∧ (Cn !!! k = t) ∧ (Cn !!! k > 0).
 
-  Definition outflow_constraint_R (Rn: inset_flowint_ur K) (es: esT) n : iProp := 
-    ⌜∀ n' k, in_outset K k Rn n' ↔ k ∈ es !!! n' ∧ in_inset K k Rn n⌝.
+  Definition outflow_constraint_R (Rn: inset_flowint_ur K) (es: esT) n := 
+    ∀ n' k, in_outset K k Rn n' ↔ k ∈ es !!! n' ∧ in_inset K k Rn n.
 
-  Definition map_of_set : gset KT → gmap K nat.
-  Proof. Admitted.
+  Definition map_of_set (C: gset KT) : gmap K nat := 
+              let C' := gset_to_gmap (0: nat) C in
+              let f := λ (kt: KT) (_: nat) M, if (M !!! kt.1 <? kt.2) 
+                                 then <[kt.1 := kt.2]> M else M in
+              map_fold f (∅: gmap K nat) C'.
 
-  Definition set_of_map : gmap K nat → gset KT.
-  Proof. Admitted.
+  Definition set_of_map (C: gmap K nat) : gset KT := 
+             let f := λ k t H, H ∪ {[(k,t)]} in
+             map_fold f (∅: gset KT) C.
 
-  Definition φ1 (Bn Cn: gmap K natUR) (In: KT_flowint_ur K) : iProp := 
-              ⌜∀ k, out_KT In k ∨ (Bn !!! k = Cn !!! k)⌝.
+  Definition φ0 (Bn: gmap K natUR) (T: nat) := 
+              ∀ k, Bn !!! k ≤ T.  
 
-  Definition φ2 n (Bn: gmap K natUR) In : iProp := 
-              ⌜∀ k t, (k,t) ∈ inset_KT In n → Bn !!! k = t⌝.
+  Definition φ1 (Bn Cn: gmap K natUR) (In: KT_flowint_ur K) := 
+              ∀ k, out_KT In k ∨ (Bn !!! k = Cn !!! k).
 
-  Definition φ3 n (Bn: gmap K natUR) Jn : iProp :=
-              ⌜∀ k t, (k,t) ∈ inset_KT Jn n → Bn !!! k ≤ t⌝.
+  Definition φ2 n (Bn: gmap K natUR) In := 
+              ∀ k t, (k,t) ∈ inset_KT In n → Bn !!! k = t.
 
-  Definition φ4 n (Bn: gmap K natUR) Rn : iProp :=
-              ⌜∀ k, Bn !! k = None ∨ in_inset K k Rn n⌝.
+  Definition φ3 n (Bn: gmap K natUR) Jn :=
+              ∀ k t, (k,t) ∈ inset_KT Jn n → Bn !!! k ≤ t.
 
-  Definition φ5 n (Rn: inset_flowint_ur K) : iProp := ⌜∀ k, inf Rn n !1 k ≤ 1⌝.
+  Definition φ4 n (Bn: gmap K natUR) Rn :=
+              ∀ k, Bn !!! k = 0 ∨ in_inset K k Rn n.
 
-  Definition maxTS (t: nat) (H: gset KT) : iProp := 
-              ⌜∀ (k: K) t', (k, t') ∈ H → t' < t⌝.
+  Definition φ5 n (Rn: inset_flowint_ur K) := 
+              ∀ k, nzmap_total_lookup k (inf Rn n) ≤ 1.
+
+  Definition maxTS (t: nat) (H: gset KT) := 
+              (∀ (k: K) t', (k, t') ∈ H → t' < t) ∧ (t > 0).
 
   Definition MCS_auth (γ_te γ_he: gname) (t: nat) (H: gset KT) : iProp := 
       own γ_te (● Excl' t) ∗ own γ_he (● Excl' H).
@@ -233,9 +246,9 @@ Section multicopy.
     ∗ ⌜domm Rn = {[n]}⌝.
     
   Definition outflow_constraints n In Jn Rn es Cn Bn : iProp :=
-      outflow_constraint_I In es Cn Bn
-    ∗ outflow_constraint_J Jn es Cn Bn
-    ∗ outflow_constraint_R Rn es n.
+      ⌜outflow_constraint_I In es Cn Bn⌝
+    ∗ ⌜outflow_constraint_J Jn es Cn Bn⌝
+    ∗ ⌜outflow_constraint_R Rn es n⌝.
       
   Definition nodePred γ_e γ_c γ_b γ_t γ_s r n (Cn Bn : gmap K natUR) : iProp :=
     ∃ es t,
@@ -245,18 +258,18 @@ Section multicopy.
     ∗ (if (n =? r) then own γ_t (●{1/2} MaxNat t) else ⌜True⌝)%I.
 
   Definition nodeShared γ_I γ_J γ_R γ_e γ_c γ_b γ_f γ_cir
-                              r n (Cn Bn : gmap K natUR) H : iProp :=
+                              r n (Cn Bn : gmap K natUR) t H : iProp :=
     ∃ es In Jn Rn,                          
       frac_ghost_state γ_e γ_c γ_b n es Cn Bn    
     ∗ singleton_interfaces_ghost_state γ_I γ_J γ_R n In Jn Rn
     ∗ inFP γ_f n
     ∗ closed γ_f es
     ∗ outflow_constraints n In Jn Rn es Cn Bn
-    ∗ (if (n =? r) then ⌜Bn = map_of_set H⌝ ∗ inflow_zero In ∗ inflow_zero Jn 
+    ∗ (if (n =? r) then ⌜Bn = map_of_set H⌝ ∗ ⌜inflow_zero In⌝ ∗ ⌜inflow_zero Jn⌝ 
                    else True)%I
     ∗ ([∗ set] k ∈ KS, own (γ_cir n k) (● (MaxNat (Bn !!! k))))
-    ∗ φ1 Bn Cn In ∗ φ2 n Bn In 
-    ∗ φ3 n Bn Jn ∗ φ4 n Bn Rn ∗ φ5 n Rn. 
+    ∗ ⌜φ0 Bn t⌝ ∗ ⌜φ1 Bn Cn In⌝ ∗ ⌜φ2 n Bn In⌝ 
+    ∗ ⌜φ3 n Bn Jn⌝ ∗ ⌜φ4 n Bn Rn⌝ ∗ ⌜φ5 n Rn⌝. 
     
   Definition global_state γ_te γ_he γ_s γ_t γ_I γ_J γ_R γ_f r t H I J R : iProp :=
       MCS_auth γ_te γ_he t H
@@ -266,9 +279,9 @@ Section multicopy.
     ∗ own γ_J (● J)
     ∗ own γ_R (● R)
     ∗ own γ_f (● domm I)
-    ∗ inflow_zero I ∗ inflow_zero J ∗ inflow_R R r
+    ∗ ⌜inflow_zero I⌝ ∗ ⌜inflow_zero J⌝ ∗ ⌜inflow_R R r⌝
     ∗ inFP γ_f r
-    ∗ maxTS t H
+    ∗ ⌜maxTS t H⌝
     ∗ ⌜domm I = domm J⌝ ∗ ⌜domm I = domm R⌝.
        
   Definition mcs γ_te γ_he γ_s γ_t γ_I γ_J γ_R γ_f γ_e γ_c γ_b γ_cir r : iProp :=
@@ -277,7 +290,7 @@ Section multicopy.
     ∗ ([∗ set] n ∈ (domm I), ∃ (bn: bool) Cn Bn, 
           lockLoc n ↦ #bn
         ∗ (if bn then True else nodePred γ_e γ_c γ_b γ_t γ_s r n Cn Bn)
-        ∗ nodeShared γ_I γ_J γ_R γ_e γ_c γ_b γ_f γ_cir r n Cn Bn H)%I.  
+        ∗ nodeShared γ_I γ_J γ_R γ_e γ_c γ_b γ_f γ_cir r n Cn Bn t H)%I.  
 
   Instance mcs_timeless γ_te γ_he γ_s γ_t γ_I γ_J γ_R γ_f γ_e γ_c γ_b γ_cir r :
     Timeless (mcs γ_te γ_he γ_s γ_t γ_I γ_J γ_R γ_f γ_e γ_c γ_b γ_cir r).
@@ -436,24 +449,55 @@ Section multicopy.
   iModIntro. iFrame.
   Qed.
 
+  Definition f_ins (k: K) (t: nat) : KT → nat → nat → nat :=
+              λ k' a1 _, if (decide (k' = (k,t))) then 1 else a1.
+
+  Definition fn (m: KT_multiset K) (n: Node) : 
+            Node → (KT_multiset K) → (KT_multiset K) → (KT_multiset K) := 
+              λ k' a1 _, if (decide (k' = n)) then m else a1.
+
+  Instance fn_id m n : ∀ k', UnitId (KT_multiset K) _ (fn m n k').
+  Proof.
+  Admitted. 
+
+(*
+  Instance nonzero_one : NonZero nat _ 1.
+  Proof.
+    unfold NonZero.
+    try done.
+  Qed.
+  
+  Instance nonzero_KT k t m : NonZero (KT_multiset K) _ (nzmap_insert (k,t) 1 m).
+  Proof.
+  Admitted.
+
+  Definition outflow_insert_KT (I : KT_flowint_ur K) (n: Node) 
+                              (k: K) (t: nat) :KT_flowint_ur K := 
+             let I_out_n := (nzmap_insert (k,t) 1 (out I n): (KT_multiset K)) in
+             let I'_out := (nzmap_insert n I_out_n (out_map I) : 
+                                      (nzmap Node (KT_multiset K))) in
+             (int {| infR := inf_map I ; outR := I'_out |}).              
+
+*)
+
   Definition outflow_insert_KT (I : KT_flowint_ur K) (n: Node) 
                               (k: K) (t: nat) :KT_flowint_ur K := 
              let I_out_n := ((nzmap_imerge 
-                         (λ k' a1 _, if (decide (k' = (k, t))) then 1 else a1)
-                         (out I n) (∅)): (KT_multiset)) in
+                             (f_ins k t)
+                             (out I n) (∅)): (KT_multiset K)) in
              let I'_out := ((nzmap_imerge 
-                          (λ k' a1 _, if (decide (k = n)) then I_out_n else a1)
-                          (out_map I) (∅)) : (nzmap Node KT_multiset)) in
+                          (fn I_out_n n)
+                          (out_map I) (∅)) : (nzmap Node (KT_multiset K))) in
              (int {| infR := inf_map I ; outR := I'_out |}).              
 
   Definition outflow_delete_KT (I : KT_flowint_ur K) (n: Node) 
                               (k: K) (t: nat) :KT_flowint_ur K := 
              let I_out_n := ((nzmap_imerge 
                          (λ k' a1 _, if (decide (k' = (k, t))) then 0 else a1)
-                         (out I n) (∅)): (KT_multiset)) in
+                         (out I n) (∅)): (KT_multiset K)) in
              let I'_out := ((nzmap_imerge 
                           (λ k' a1 _, if (decide (k = n)) then I_out_n else a1)
-                          (out_map I) (∅)) : (nzmap Node KT_multiset)) in
+                          (out_map I) (∅)) : (nzmap Node (KT_multiset K))) in
              (int {| infR := inf_map I ; outR := I'_out |}).
 
   Lemma outflow_insert_outset_KT I n k t I' :
@@ -461,6 +505,12 @@ Section multicopy.
            ∀ n', (n' = n → outset_KT I' n' = (outset_KT I n') ∪ {[(k,t)]})
                ∧ (n' ≠ n → outset_KT I' n' = outset_KT I n').
   Proof.
+    intros Heq n'. split.
+    - intros Hn; replace n'.
+      unfold outset_KT.
+      unfold KT_flows.dom_ms.
+      replace I'. unfold outflow_insert_KT.
+      unfold out at 1. simpl. 
   Admitted.
 
   Lemma outflow_delete_outset_KT I n k t I' :
@@ -474,26 +524,26 @@ Section multicopy.
                               (k: K) (t: nat) :KT_flowint_ur K := 
              let I_inf_n := ((nzmap_imerge 
                          (λ k' a1 _, if (decide (k' = (k, t))) then 1 else a1)
-                         (inf I n) (∅)): (KT_multiset)) in
-             let I'_inf := (<[ n := I_inf_n ]>(inf_map I):(gmap Node KT_multiset)) in
+                         (inf I n) (∅)): (KT_multiset K)) in
+             let I'_inf := (<[ n := I_inf_n ]>(inf_map I)) in
              (int {| infR := I'_inf ; outR := out_map I |}).              
 
   Definition inflow_delete_KT (I : KT_flowint_ur K) (n: Node) 
                               (k: K) (t: nat) :KT_flowint_ur K := 
              let I_inf_n := ((nzmap_imerge 
                          (λ k' a1 _, if (decide (k' = (k, t))) then 0 else a1)
-                         (inf I n) (∅)): (KT_multiset)) in
-             let I'_inf := (<[ n := I_inf_n ]>(inf_map I):(gmap Node KT_multiset)) in
+                         (inf I n) (∅))) in
+             let I'_inf := (<[ n := I_inf_n ]>(inf_map I)) in
              (int {| infR := I'_inf ; outR := out_map I |}).           
 
-  Lemma inflow_insert_outset_KT I n k t I' :
+  Lemma inflow_insert_inset_KT I n k t I' :
         I' = inflow_insert_KT I n k t → 
            ∀ n', (n' = n → inset_KT I' n' = (inset_KT I n') ∪ {[(k,t)]})
                ∧ (n' ≠ n → inset_KT I' n' = inset_KT I n').
   Proof.
   Admitted.
 
-  Lemma inflow_delete_outset_KT I n k t I' :
+  Lemma inflow_delete_inset_KT I n k t I' :
         I' = inflow_delete_KT I n k t → 
            ∀ n', (n' = n → inset_KT I' n' = (inset_KT I n') ∖ {[(k,t)]})
                ∧ (n' ≠ n → inset_KT I' n' = inset_KT I n').
@@ -575,9 +625,33 @@ Section multicopy.
     done.
   Admitted.
 
+  Lemma set_of_map_insert_subseteq (C: gmap K nat) k t H :
+        set_of_map C = H → 
+            set_of_map (<[k := t]> C) ⊆ H ∪ {[(k, t)]}.
+  Proof.
+  Admitted.          
+
+  Lemma set_of_map_member (C: gmap K nat) k t :
+            C !! k = Some(t) →    
+              (k, t) ∈ set_of_map C.
+  Proof.
+  Admitted.
+  
+  Lemma map_of_set_insert_eq (C: gmap K nat) k T H :
+        (∀ t, (k, t) ∈ H → t < T) → 
+                  C = map_of_set H →
+                 <[k := T]> C = map_of_set (H ∪ {[(k, T)]}).
+  Proof.
+  Admitted.
+
+  Lemma outflow_constraint_outset_I In es Cn Bn : 
+        ∀ k, outflow_constraint_I In es Cn Bn →
+                Cn !!! k ≠ 0 → ¬ out_KT In k.
+  Proof.
+  Admitted.
+
 
   (** Proofs **)  
-
 
 (*
   Lemma traverse_spec γ_te γ_he γ_s γ_t γ_I γ_J γ_R 
@@ -618,7 +692,7 @@ Section multicopy.
                                 & HnS_cl & HnS_oc & HnS_H & HnS_star & Hφ)".
         iPoseProof (frac_eq with "[$HnP_frac] [$HnS_frac]") as "%".
         destruct H1 as [Hes [Hc Hb]]. subst es'. subst Cn'. subst Bn'.
-        iAssert (inFP γ_f n1)%I as "#HFP_n1".
+        iAssert (inFP γ_f n1)%I as "#FP_n1".
         { iApply "HnS_cl". iPureIntro. 
           clear -k_in_es. set_solver. }
         iAssert (⌜(k, Bn !!! k) ∈ outset_KT In n1⌝)%I as %outflow_n_n1.
@@ -628,8 +702,14 @@ Section multicopy.
           repeat split; try done. apply bool_decide_eq_true in Ht.
           inversion Ht as [H'']. rewrite Cn_val. admit. }
         iAssert (⌜n1 ∈ domm I⌝)%I as %n_in_I.
-        { admit. }
-        rewrite (big_sepS_delete _ (domm I ∖ {[n]}) n1); last admit.
+        { iDestruct "Hglob" as "(_ & _ & _ & _ & _ & _ & Hf & _)". 
+          by iPoseProof (inFP_domm _ _ _ with "[$FP_n1] [$Hf]") as "H'". }
+        iAssert (⌜n ≠ n1⌝)%I as %n_neq_n1.
+        { destruct (decide (n = n1)); try done.
+          iPoseProof (node_edgeset_self_empty with "node_n") as "%".
+          rename H1 into Es_n. rewrite <-e in k_in_es.
+          clear -k_in_es Es_n. set_solver. } 
+        rewrite (big_sepS_delete _ (domm I ∖ {[n]}) n1); last by set_solver.
         iDestruct "Hstar'" as "(H_n1 & Hstar'')".
         iDestruct "H_n1" as (bn1 Cn1 Bn1)"(Hl_n1 & Hlif_n1 & HnS_n1)".
         iDestruct "HnS_n1" as (es1 In1 Jn1 Rn1) 
@@ -638,7 +718,8 @@ Section multicopy.
         iAssert (⌜(k, Bn !!! k) ∈ inset_KT In1 n1⌝)%I as %inflow_n1.
         { admit. }
         iAssert (⌜Bn1 !!! k = Bn !!! k⌝)%I as %Bn1_eq_Bn.
-        { admit. }
+        { iDestruct "Hφ1" as "(_ & % & _)". rename H1 into Hφ2.
+          by pose proof Hφ2 k (Bn !!! k) inflow_n1. } 
         iEval (rewrite (big_sepS_elem_of_acc (_) (KS) k); last by eauto) 
                                                                 in "HnS_star".
         iDestruct "HnS_star" as "(Hcirk_n & HnS_star')".
@@ -662,7 +743,7 @@ Section multicopy.
         iExists bn1, Cn1, Bn1. iFrame "Hl_n1 Hlif_n1".
         iExists es1, In1, Jn1, Rn1. iFrame. by iApply "HnS_star1'".
         iModIntro.        
-        awp_apply (unlockNode_spec_high with "[] [] [HnP_n' node_n]"); 
+        awp_apply (unlockNode_spec_high with "[] [] [HnP_n' node_r]"); 
                         try done. iExists es, T. iFrame.                
         iAaccIntro with ""; try eauto with iFrame.
         iIntros "_". iModIntro. wp_pures.
@@ -706,13 +787,13 @@ Section multicopy.
         iMod "AU" as (t' H') "[MCS [_ Hclose]]". iSpecialize ("Hclose" $! 0).
         iMod ("Hclose" with "[MCS]") as "HΦ". iFrame. 
         iPureIntro. split; try done. admit.
-        iModIntro. iSplitR "node_n HnP_n' HΦ". iNext.
+        iModIntro. iSplitR "node_r HnP_n' HΦ". iNext.
         iExists T', H, I, J, R. iFrame "Hglob".
         rewrite (big_sepS_delete _ (domm I) n); last by eauto.
         iFrame "Hstar'". iExists bn, Cn, Bn.
         iFrame "Hl_n Hlif_n". iExists es, In, Jn, Rn.
         iFrame "∗%". by iApply "HnS_star'". iModIntro.
-        awp_apply (unlockNode_spec_high with "[] [] [HnP_n' node_n]") without "HΦ";
+        awp_apply (unlockNode_spec_high with "[] [] [HnP_n' node_r]") without "HΦ";
                         try done. iExists es, T. iFrame.
         iAaccIntro with ""; try eauto with iFrame.
         iIntros "_". iModIntro. iIntros "HΦ". by wp_pures.
@@ -759,13 +840,13 @@ Section multicopy.
       iMod ("Hclose" with "[MCS]") as "HΦ". iFrame. 
       iPureIntro. split. set_solver. rewrite Hφ1 in lb_t1.
       rewrite Cn_val in lb_t1. lia.
-      iModIntro. iSplitR "node_n HnP_n' HΦ". iNext.
+      iModIntro. iSplitR "node_r HnP_n' HΦ". iNext.
       iExists T', H, I, J, R. iFrame "Hglob".
       rewrite (big_sepS_delete _ (domm I) n); last by eauto.
       iFrame "Hstar'". iExists bn, Cn, Bn.
       iFrame "Hl_n Hlif_n". iExists es, In, Jn, Rn.
       iFrame "∗%". by iApply "HnS_star'". iModIntro.
-      awp_apply (unlockNode_spec_high with "[] [] [HnP_n' node_n]") without "HΦ"; 
+      awp_apply (unlockNode_spec_high with "[] [] [HnP_n' node_r]") without "HΦ"; 
                       try done. iExists es, T. iFrame.
       iAaccIntro with ""; try eauto with iFrame.
       iIntros "_". iModIntro. iIntros "HΦ". by wp_pures.
@@ -793,12 +874,12 @@ Section multicopy.
     awp_apply lockNode_spec_high; try done.
     iAaccIntro with ""; try eauto with iFrame. 
     iIntros (Cr Br)"HnP_n". iModIntro. wp_pures.
-    iDestruct "HnP_n" as (es T)"(node_n & HnP_frac & HnP_C & HnP_t)".
+    iDestruct "HnP_n" as (es T)"(node_r & HnP_frac & HnP_C & HnP_t)".
     iEval (rewrite <-beq_nat_refl) in "HnP_t".
     wp_apply (readClock_spec with "[HnP_t]"); try done.
     iIntros "HnP_t". wp_pures.
-    wp_apply (addContents_spec with "node_n").
-    iIntros (b Cr')"(node_n & Hif)".
+    wp_apply (addContents_spec with "node_r").
+    iIntros (b Cr')"(node_r & Hif)".
     destruct b; last first.
     - iDestruct "Hif" as %HCr. replace Cr'. wp_pures.
       awp_apply (unlockNode_spec_high with "[] [] [-AU]"); try done.
@@ -820,22 +901,49 @@ Section multicopy.
       { iCombine "Ht HnP_t" as "H'". done. }          
       iAaccIntro with "H".
       { iIntros "H". iDestruct "H" as "(Ht & HnP_t)".
-        iModIntro. iSplitR "AU HnP_frac HnP_C node_n HnP_t".
+        iModIntro. iSplitR "AU HnP_frac HnP_C node_r HnP_t".
         iNext. iExists T, H1, I1, J1, R1. iFrame "∗ #". iFrame. }
       iIntros "H". iDestruct "H" as "(Ht & HnP_t)".
-      iMod (own_update γ_s (● H1) (● (H1 ∪ {[(k,T)]})) with "[$HH]") as "HH".
-      { apply (auth_update_auth _ _ (H1 ∪ {[(k,T)]})).
-        apply gset_local_update. set_solver. } 
-      iAssert (maxTS (T+1) (H1 ∪ {[(k, T)]}))%I with "[Max_ts]" as "Max_ts".
-      { iDestruct "Max_ts" as %Max_ts. iPureIntro. intros k' t' H.
+      iPoseProof ((auth_own_incl γ_s H1 _) with "[$HH $HnP_C]") as "%".
+      rename H into Cr_sub_H1. apply gset_included in Cr_sub_H1.
+      iDestruct "Max_ts" as %Max_tsH1.
+      assert (maxTS (T+1) (H1 ∪ {[(k, T)]})) as Max_ts.
+      { split. intros k' t' H.
         assert (((k',t') ∈ H1) ∨ (k' = k ∧ t' = T)) as Hor by set_solver.
         destruct Hor as [Hor | Hor]. 
-          pose proof Max_ts k' t' Hor as Hres. lia.
-          destruct Hor as [_ Hor]. replace t'. lia. }       
-      iAssert (⌜set_of_map Cr ⊆ set_of_map Cr'⌝)%I as %Cr_sub_Cr'.
-      { admit. }
-      iAssert (own γ_s (◯ set_of_map Cr'))%I with "[HnP_C]" as "HnP_C".
-      { admit. }
+        destruct Max_tsH1 as [Max_tsH1 _].
+        pose proof Max_tsH1 k' t' Hor as Hres. lia.
+        destruct Hor as [_ Hor]. replace t'. lia.
+        destruct Max_tsH1 as [_ Max_tsH1]. lia. }       
+      iAssert (⌜set_of_map Cr' ⊆ H1 ∪ {[(k,T)]}⌝)%I as %Cr_sub_H1'.
+      { iPureIntro. replace Cr'.
+        pose proof (set_of_map_insert_subseteq Cr k T (set_of_map Cr)) as H'.
+        assert (set_of_map Cr = set_of_map Cr) as H'' by done. 
+        apply H' in H''.
+        intros x Hx. clear -Cr_sub_H1 H'' Hx. set_solver.
+         }
+      iMod (own_update γ_s (● H1) (● (H1 ∪ {[(k,T)]})) with "[$HH]") as "HH".
+      { apply (auth_update_auth _ _ (H1 ∪ {[(k,T)]})).
+        apply gset_local_update. set_solver. }
+      iMod (own_update γ_s (● (H1 ∪ {[(k, T)]})) 
+             (● (H1 ∪ {[(k, T)]}) ⋅ ◯ (set_of_map Cr')) with "[$HH]") as "HH".
+      { apply (auth_update_alloc _ (H1 ∪ {[(k,T)]}) (set_of_map Cr')).
+        apply local_update_discrete. intros m Valid_H1 H1_eq.
+        split; try done. rewrite /(ε ⋅? m) in H1_eq.
+        destruct m. rewrite gset_op_union in H1_eq. 
+        rewrite left_id in H1_eq *; intros H1_eq.
+        rewrite <-H1_eq. 
+        rewrite /(set_of_map Cr' ⋅? Some (H1 ∪ {[k, T]})).
+        rewrite gset_op_union.
+        rewrite /(ε) in H1_eq. unfold ucmra_unit in H1_eq.
+        simpl in H1_eq.
+        assert ((k,T) ∈ set_of_map Cr') as H'.
+        { replace Cr'. apply set_of_map_member.
+          apply lookup_insert. } 
+        clear - H' Cr_sub_H1 Cr_sub_H1'. set_solver.
+        exfalso. clear -H1_eq. set_solver. }
+      iDestruct "HnP_C" as "_".  
+      iDestruct "HH" as "(HH & HnP_C)".   
       iAssert (⌜r ∈ domm I1⌝)%I as %r_in_I.
       { by iPoseProof (inFP_domm _ _ _ with "[$FP_r] [$Hf]") as "H'". }
       rewrite (big_sepS_delete _ (domm I1) r); last by eauto.
@@ -851,34 +959,85 @@ Section multicopy.
                                         HnS_if & HnS_star & Hφ)".
       iPoseProof (frac_eq with "[$HnP_frac] [$HnS_frac]") as "%".
       destruct H as [Hes [Hc Hb]]. subst es'. subst Cr''. subst Br''.
-      destruct (decide (Cr !!! k = 0)) as [ Cr_k | Cr_k ]; last first.
-      + set (Br' := <[k := T]>Br).
+      set (Br' := <[k := T]>Br).
         assert (Br' = <[k := T]>Br) as HBr'. try done.
+        iEval (rewrite <-beq_nat_refl) in "HnS_if".
+        iDestruct "HnS_if" as "(H' & H'' & H''')".
+        iDestruct "H'" as %Br_eq_H1. 
+        iDestruct "H''" as %Infz_rI.
+        iDestruct "H'''" as %Infz_rJ.
         iAssert (⌜Br' = map_of_set (H1 ∪ {[(k, T)]})⌝)%I as %Br'_eq_H1.
-        { admit. }
-        assert (∀ k', k' ≠ k → Br' !!! k' = Br !!! k') as HBr_neq.
-        { intros k' Hk'. rewrite /(Br !!! k').
-          rewrite /(Br' !!! k'). 
-          unfold finmap_lookup_total.
-          unfold inhabitant. simpl.
-          assert (Br' !! k' = Br !! k') as HBr.
-          { by apply lookup_insert_ne. } 
-          by rewrite HBr. }
-        assert (Br' !!! k = T) as HBr'_k.
-        { apply lookup_total_insert. }          
-        iAssert ([∗ set] k0 ∈ KS, own (γ_cir r k0) 
-                    (● {| max_nat_car := Br' !!! k0 |}))%I 
-            with "[HnS_star]" as "HnS_star".
-        { admit. }
-        iMod ((frac_update γ_e γ_c γ_b r es Cr Br es Cr' Br') 
-                    with "[$HnP_frac $HnS_frac]") as "(HnP_frac & HnS_frac)".
-        assert ((∃ n, k ∈ es !!! n ∧ n ≠ r) ∨ (∀ n, k ∉ es !!! n)) as Hes.
-        { admit. } destruct Hes as [Hes | Hes].
-        * destruct Hes as [n [k_in_es n_neq_r]].
-          set (Jr'_temp := outflow_delete_KT Jr n k (Cr !!! k)).
-          set (Jr' := outflow_insert_KT Jr'_temp n k T).
+        { iPureIntro.
+          apply map_of_set_insert_eq; try done.
+          intros t. 
+          destruct Max_tsH1 as [Max_tsH1 _].
+          by pose proof Max_tsH1 k t. }
+      destruct (out_edgeset k es) eqn: Hes.
+      + apply out_edgeset_true in Hes.
+        destruct Hes as [n k_in_es].
+        iPoseProof (node_edgeset_self_empty with "node_r") as "%".
+        rename H into Self_es.
+        assert (n ≠ r) as n_neq_r.
+        { destruct (decide (n = r)); try done.
+          rewrite e in k_in_es.
+          clear -Self_es k_in_es.
+          set_solver. } 
+        destruct (decide (Cr !!! k  = 0)) as [ Cr_k | Cr_k ]; last first.
+        * iEval (rewrite (big_sepS_delete (_) (KS) k); last by eauto) in "HnS_star".
+          iDestruct "HnS_star" as "(Hk & HnS_star')".
+          iAssert (⌜Br !!! k ≤ T⌝)%I as %Br_le_T.
+          { iDestruct "HnS_oc" as "(% & _)". rename H into HocI.
+            pose proof outflow_constraint_outset_I Ir es Cr Br k HocI Cr_k as H'.
+            iDestruct "Hφ" as "(_ & % & _)". rename H into Hφ1.
+            pose proof Hφ1 k as Hφ1. 
+            destruct Hφ1 as [Hφ1 | Hφ1]; try done.
+            destruct (Cr !! k) eqn: Hc.
+            assert (Hc' := Hc).
+            apply set_of_map_member in Hc.
+            assert ((k,u) ∈ H1) as Hu by set_solver.
+            unfold maxTS in Max_tsH1.
+            apply Max_tsH1 in Hu.
+            iPureIntro. rewrite Hφ1. 
+            rewrite /(Cr !!! k).
+            unfold finmap_lookup_total.
+            rewrite Hc'. simpl. lia.
+            rewrite /(Cr !!! k) in Cr_k.
+            unfold finmap_lookup_total in Cr_k.
+            rewrite Hc in Cr_k. simpl in Cr_k. lia. }
+          iMod (own_update (γ_cir r k) (● (MaxNat (Br !!! k))) 
+                  (● (MaxNat (Br' !!! k))) with "Hk") as "Hk".
+          { apply (auth_update_auth _ _ (MaxNat (Br' !!! k))).
+            apply max_nat_local_update.
+            simpl. rewrite HBr'.
+            by rewrite lookup_total_insert. }        
+          iAssert ([∗ set] k0 ∈ KS, own (γ_cir r k0) 
+                      (● {| max_nat_car := Br' !!! k0 |}))%I 
+              with "[HnS_star' Hk]" as "HnS_star".
+          { iEval (rewrite (big_sepS_delete (_) (KS) k); last by eauto).
+            iFrame "Hk".        
+            iApply (big_opS_proper 
+                   (λ y, own (γ_cir r y) (● {| max_nat_car := Br' !!! y |}))
+                   (λ y, own (γ_cir r y) (● {| max_nat_car := Br !!! y |})) 
+                   (KS ∖ {[k]})).
+            intros x Hx. assert (x ≠ k) as H' by set_solver.
+            iFrame. iSplit. 
+            iIntros "H". iEval (rewrite HBr') in "H".
+            assert (<[k:=T]> Br !!! x = Br !!! x) as H''. 
+            { apply lookup_total_insert_ne; try done. } 
+            by iEval (rewrite H'') in "H".       
+            iIntros "H". iEval (rewrite HBr').
+            assert (<[k:=T]> Br !!! x = Br !!! x) as H''. 
+            { apply lookup_total_insert_ne; try done. } 
+            by iEval (rewrite H'').
+            done. }
+          iMod ((frac_update γ_e γ_c γ_b r es Cr Br es Cr' Br') 
+                      with "[$HnP_frac $HnS_frac]") as "(HnP_frac & HnS_frac)".
+          set (Jr_temp := outflow_delete_KT Jr n k (Cr !!! k)).
+          set (Jr' := outflow_insert_KT Jr_temp n k T).
+          iPoseProof (node_edgeset_disjoint with "node_r") as "%".
+          rename H into Disj_es.
           iAssert (outflow_constraints r Ir Jr' Rr es Cr' Br')%I 
-                    with "[HnS_oc]" as "HnS_oc".
+                      with "[HnS_oc]" as "HnS_oc".
           { iDestruct "HnS_oc" as "(% & % & %)".
             rename H into OC_1. rename H2 into OC_2.
             rename H3 into OC_3. 
@@ -903,7 +1062,9 @@ Section multicopy.
                 * replace k'.
                   rewrite e in Hout2. replace Cr' in Hout2.
                   rewrite lookup_total_insert in Hout2.
-                  admit. (* Contradiction: T = 0 *)
+                  clear -Max_tsH1 Hout2.
+                  destruct Max_tsH1 as [_ Max_tsH1].
+                  lia.
                 * rewrite /(Cr' !!! k') in Hout2.
                   unfold finmap_lookup_total in Hout2.
                   replace Cr' in Hout2. 
@@ -916,13 +1077,13 @@ Section multicopy.
               destruct (decide (n' = n)).
               + assert (outset_KT Jr' n = 
                       (outset_KT Jr n ∖ {[k, Cr !!! k]}) ∪ {[k, T]}) as Outset.
-                { pose proof outflow_insert_outset_KT Jr'_temp n k T Jr' as Houts.
-                  assert (Jr' = outflow_insert_KT Jr'_temp n k T) as HJr' by done.
+                { pose proof outflow_insert_outset_KT Jr_temp n k T Jr' as Houts.
+                  assert (Jr' = outflow_insert_KT Jr_temp n k T) as HJr' by done.
                   pose proof Houts HJr' n' as [Hp _].
                   pose proof Hp e as Hp.
-                  pose proof outflow_delete_outset_KT Jr n k (Cr !!! k) Jr'_temp 
+                  pose proof outflow_delete_outset_KT Jr n k (Cr !!! k) Jr_temp 
                     as Houts'. 
-                  assert (Jr'_temp = outflow_delete_KT Jr n k (Cr !!! k)) 
+                  assert (Jr_temp = outflow_delete_KT Jr n k (Cr !!! k)) 
                     as HJr_t by done.  
                   pose proof Houts' HJr_t n' as [Hp' _].
                   pose proof Hp' e as Hp'.
@@ -938,24 +1099,45 @@ Section multicopy.
                 * intros Hout. pose proof Hkt' Hout as Hkt'.
                   destruct Hkt' as [Hkt' | Hkt'].
                   ** apply OC_2 in Hkt'.
-                     destruct Hkt' as [Hkt'_1 Hkt'_2]. 
-                     split; try done.
+                     destruct Hkt' as [Hkt'_1 [Hkt'_2 Hkt'_3]]. 
+                     split; try done. split.
                      destruct (decide (k' = k)).
                      rewrite e0 in Hkt'_2.
                      rewrite e0 in Hout.
                      rewrite <-Hkt'_2 in Hout.
                      assert ((k, Cr !!! k) ∉ outset_KT Jr' n).
-                     { clear -Outset.
-                       assert (Cr !!! k ≠ T). admit.
-                       set_solver. }
+                     { destruct (Cr !! k) eqn: Hc.
+                       assert (Hc' := Hc).
+                       apply set_of_map_member in Hc.
+                       assert ((k,u) ∈ H1) as H' by set_solver.
+                       destruct Max_tsH1 as [Max_tsH1 _].
+                       apply Max_tsH1 in H'.
+                       assert (Cr !!! k ≠ T).
+                       rewrite /(Cr !!! k).
+                       unfold finmap_lookup_total.
+                       rewrite Hc'. simpl. lia.
+                       set_solver.
+                       rewrite /(Cr !!! k) in Cr_k.
+                       unfold finmap_lookup_total in Cr_k.
+                       rewrite Hc in Cr_k. simpl in Cr_k. lia. }
                      contradiction.
                      replace Cr'. 
+                     rewrite lookup_total_insert_ne; try done.
+                     destruct (decide (k' = k)).
+                     rewrite e0.
+                     replace Cr'.
+                     rewrite lookup_total_insert. 
+                     by destruct Max_tsH1 as [_ H'].
+                     replace Cr'.
                      rewrite lookup_total_insert_ne; try done.
                   ** inversion Hkt'.
                      repeat split; try done.
                      replace Cr'.
                      rewrite lookup_total_insert; try done.
-                * intros [Hk1 Hk2].
+                     replace Cr'.
+                     rewrite lookup_total_insert. 
+                     by destruct Max_tsH1 as [_ H'].
+                * intros [Hk1 [Hk2 Hk3]].
                   destruct (decide (k' = k)).
                   ** replace k'.
                      rewrite e0 in Hk1.
@@ -966,18 +1148,21 @@ Section multicopy.
                      set_solver.
                   ** replace Cr' in Hk2.
                      rewrite lookup_total_insert_ne in Hk2; try done.
-                     assert (k' ∈ es !!! n ∧ Cr !!! k' = t') as Hkt; try done.
+                     replace Cr' in Hk3.
+                     rewrite lookup_total_insert_ne in Hk3; try done.
+                     assert (k' ∈ es !!! n ∧ Cr !!! k' = t' ∧ Cr !!! k' > 0) 
+                                        as Hkt; try done.
                      apply OC_2 in Hkt.
                      rewrite Outset.
                      clear -Hkt n0. set_solver.
               + assert (outset_KT Jr' n' = outset_KT Jr n') as Outset.
-                { pose proof outflow_insert_outset_KT Jr'_temp n k T Jr' as Houts.
-                  assert (Jr' = outflow_insert_KT Jr'_temp n k T) as HJr' by done.
+                { pose proof outflow_insert_outset_KT Jr_temp n k T Jr' as Houts.
+                  assert (Jr' = outflow_insert_KT Jr_temp n k T) as HJr' by done.
                   pose proof Houts HJr' n' as [_ Hp].
                   pose proof Hp n0 as Hp.
-                  pose proof outflow_delete_outset_KT Jr n k (Cr !!! k) Jr'_temp 
+                  pose proof outflow_delete_outset_KT Jr n k (Cr !!! k) Jr_temp 
                     as Houts'. 
-                  assert (Jr'_temp = outflow_delete_KT Jr n k (Cr !!! k)) 
+                  assert (Jr_temp = outflow_delete_KT Jr n k (Cr !!! k)) 
                     as HJr_t by done.  
                   pose proof Houts' HJr_t n' as [_ Hp'].
                   pose proof Hp' n0 as Hp'.
@@ -986,24 +1171,30 @@ Section multicopy.
                 split.
                 * intros Hout.
                   apply OC_2 in Hout.
-                  destruct Hout as [Hout1 Hout2].
+                  destruct Hout as [Hout1 [Hout2 Hout3]].
                   split; try done.
                   destruct (decide (k' = k)).
                   ** rewrite e in Hout1.
-                     admit.
+                     pose proof Disj_es n' n n0 as H'.
+                     clear -H' Hout1 k_in_es. 
+                     set_solver.
                   ** replace Cr'.
                      rewrite lookup_total_insert_ne; try done.
-                * intros [Hout1 Hout2].
+                * intros [Hout1 [Hout2 Hout3]].
                   destruct (decide (k' = k)).
                   ** rewrite e in Hout1.
-                     admit.
+                     pose proof Disj_es n' n n0 as H'.
+                     clear -H' Hout1 k_in_es. 
+                     set_solver.
                   ** replace Cr' in Hout2.
                      rewrite lookup_total_insert_ne in Hout2; try done.
+                     replace Cr' in Hout3.
+                     rewrite lookup_total_insert_ne in Hout3; try done.
                      apply OC_2.
                      split; try done. }
           iAssert (inFP γ_f n)%I as "#FP_n".
           { iApply "HnS_cl". iPureIntro.
-            clear -k_in_es. set_solver. }
+          clear -k_in_es. set_solver. }
           iAssert (⌜n ∈ domm I1⌝)%I as %n_in_I.
           { by iPoseProof (inFP_domm _ _ _ with "[$FP_n] [$Hf]") as "H'". }
           rewrite (big_sepS_delete _ (domm I1 ∖ {[r]}) n); last by set_solver.
@@ -1012,8 +1203,8 @@ Section multicopy.
           iDestruct "HnS_n" as (es_n In Jn Rn) 
             "(HnS_fracn & HnS_sin & HnS_FPn & HnS_cln & HnS_ocn & 
                                         HnS_ifn & HnS_starn & Hφn)".
-          set (Jn'_temp := inflow_delete_KT Jn n k (Cr !!! k)).
-          set (Jn' := inflow_insert_KT Jn'_temp n k T).
+          set (Jn_temp := inflow_delete_KT Jn n k (Cr !!! k)).
+          set (Jn' := inflow_insert_KT Jn_temp n k T).
           iAssert (outflow_constraints n In Jn' Rn es_n Cn Bn)%I
             with "[HnS_ocn]" as "HnS_ocn".
           { iDestruct "HnS_ocn" as "(% & % & %)".
@@ -1027,32 +1218,27 @@ Section multicopy.
             iDestruct "HnS_si" as "(HrI & HrJ & HrR & Domm_rI & Domm_rJ & Domm_rR)".
             iDestruct "HnS_sin" as "(HnI & HnJ & HnR & Domm_nI & Domm_nJ & Domm_nR)".
             assert (domm Jn' = domm Jn).
-            { assert (Jn'_temp = inflow_delete_KT Jn n k (Cr !!! k)) 
+            { assert (Jn_temp = inflow_delete_KT Jn n k (Cr !!! k)) 
                           as HJn't by done.
-              assert (Jn' = inflow_insert_KT Jn'_temp n k T) as HJn' by done.
-              assert (domm Jn' = domm Jn'_temp) as H'.
+              assert (Jn' = inflow_insert_KT Jn_temp n k T) as HJn' by done.
+              assert (domm Jn' = domm Jn_temp) as H'.
               apply (inflow_insert_domm _ n k T); try done.
-              assert (domm Jn'_temp = domm Jn) as H''.
+              assert (domm Jn_temp = domm Jn) as H''.
               apply (inflow_delete_domm _ n k (Cr !!! k)); try done.
               by rewrite H'. } 
             rewrite H. iFrame.
             iCombine "HrJ HnJ" as "HrnJ".
             assert (Jr ⋅ Jn = Jr' ⋅ Jn') as H'.
-            { assert (Jr ⋅ Jn = Jr'_temp ⋅ Jn'_temp) as H'.
-              { apply (flow_delete_eq_KT Jr Jr'_temp _ _ n k (Cr !!! k));
-                         try done. }
-              assert (Jr'_temp ⋅ Jn'_temp = Jr' ⋅ Jn') as H''.
-              { apply (flow_insert_eq_KT Jr'_temp Jr' _ _ n k T);
+            { assert (Jr ⋅ Jn = Jr_temp ⋅ Jn_temp) as H'.
+              { apply (flow_delete_eq_KT Jr Jr_temp _ _ n k (Cr !!! k));
+                        try done. }
+              assert (Jr_temp ⋅ Jn_temp = Jr' ⋅ Jn') as H''.
+              { apply (flow_insert_eq_KT Jr_temp Jr' _ _ n k T);
                          try done. }
               by rewrite H'. }            
             iEval (rewrite H') in "HrnJ".
             iEval (rewrite auth_frag_op) in "HrnJ".
             iDestruct "HrnJ" as "(HrJ & HnJ)". iFrame. }
-          iEval (rewrite <-beq_nat_refl) in "HnS_if".
-          iDestruct "HnS_if" as "(H' & H'' & H''')".
-          iDestruct "H'" as %Br_eq_H1. 
-          iDestruct "H''" as %Infz_rI.
-          iDestruct "H'''" as %Infz_rJ.
           iDestruct "Inf_R" as %Inf_R.
           iPoseProof ((auth_own_incl γ_R R1 Rr) with "[HR HnS_si]")
               as (Ro) "%". 
@@ -1064,11 +1250,16 @@ Section multicopy.
           iAssert (⌜domm Rr = {[r]}⌝)%I as "%".
           { by iDestruct "HnS_si" as "(_&_&_&_&_&H')". }
           rename H into Domm_Rr.
-          iAssert (φ1 Br' Cr' Ir ∗ φ2 r Br' Ir ∗ φ3 r Br' Jr' ∗ φ4 r Br' Rr 
-                  ∗ φ5 r Rr)%I with "[Hφ]" as "Hφ".
+          iAssert (⌜φ0 Br' (T+1)⌝ ∗ ⌜φ1 Br' Cr' Ir⌝ ∗ ⌜φ2 r Br' Ir⌝ ∗ ⌜φ3 r Br' Jr'⌝ 
+                  ∗ ⌜φ4 r Br' Rr⌝ ∗ ⌜φ5 r Rr⌝)%I with "[Hφ]" as "Hφ".
           { iDestruct "Hφ" as %Hφ. 
-            destruct Hφ as [Hφ1 [Hφ2 [Hφ3 [Hφ4 Hφ5]]]].
+            destruct Hφ as [Hφ0 [Hφ1 [Hφ2 [Hφ3 [Hφ4 Hφ5]]]]].
             iPureIntro. repeat split; try done.
+            - intros k'. destruct (decide (k' = k)).
+              rewrite HBr'. rewrite e. rewrite lookup_total_insert. lia.
+              rewrite HBr'. rewrite lookup_total_insert_ne; try done.
+              pose proof Hφ0 k' as H'. clear -H'. Search (≤). 
+              apply (Nat.le_trans _ T _); try done. lia. 
             - intros k'. pose proof Hφ1 k' as Hφ1.
               destruct Hφ1 as [Hφ1 | Hφ1].
               by left.
@@ -1088,9 +1279,9 @@ Section multicopy.
             - intros k' t' Hins.
               pose proof Infz_rJ r as Infz_rJ.
               assert (inset_KT Jr' r = inset_KT Jr r) as H'.
-              { assert (inset_KT Jr'_temp r = inset_KT Jr r) as H'.
+              { assert (inset_KT Jr_temp r = inset_KT Jr r) as H'.
                 apply (outflow_delete_inf_eq_KT _ n k (Cr !!! k)); try done.
-                assert (inset_KT Jr' r = inset_KT Jr'_temp r) as H''.
+                assert (inset_KT Jr' r = inset_KT Jr_temp r) as H''.
                 apply (outflow_insert_inf_eq_KT _ n k T); try done.
                 by rewrite <-H'. }
               rewrite H' in Hins. rewrite Infz_rJ in Hins.
@@ -1101,34 +1292,35 @@ Section multicopy.
               pose proof Inf_R r k' as Inf_R.
               by rewrite <-beq_nat_refl in Inf_R.
               rewrite Domm_Rr. clear. set_solver. } 
-          iAssert (φ1 Bn Cn In ∗ φ2 n Bn In ∗ φ3 n Bn Jn' ∗ φ4 n Bn Rn 
-                  ∗ φ5 n Rn)%I with "[Hφn]" as "Hφn".
+          iAssert (⌜φ0 Bn (T+1)⌝ ∗ ⌜φ1 Bn Cn In⌝ ∗ ⌜φ2 n Bn In⌝ ∗ ⌜φ3 n Bn Jn'⌝ 
+                  ∗ ⌜φ4 n Bn Rn⌝ ∗ ⌜φ5 n Rn⌝)%I with "[Hφn]" as "Hφn".
           { iDestruct "Hφn" as %Hφ. 
-            destruct Hφ as [Hφ1 [Hφ2 [Hφ3 [Hφ4 Hφ5]]]].
+            destruct Hφ as [Hφ0 [Hφ1 [Hφ2 [Hφ3 [Hφ4 Hφ5]]]]].
             iPureIntro. repeat split; try done.
+            intros k'. pose proof Hφ0 k' as H'.
+            apply (Nat.le_trans _ T _); try done. lia. 
             intros k' t'. 
             assert (inset_KT Jn' n = 
                       (inset_KT Jn n ∖ {[k, Cr !!! k]}) ∪ {[k, T]}) as Inset.
-            { pose proof inflow_insert_outset_KT Jn'_temp n k T Jn' as Hin.
-              assert (Jn' = inflow_insert_KT Jn'_temp n k T) as HJn' by done.
+            { pose proof inflow_insert_inset_KT Jn_temp n k T Jn' as Hin.
+              assert (Jn' = inflow_insert_KT Jn_temp n k T) as HJn' by done.
               pose proof Hin HJn' n as [Hp _].
               assert (n = n) as H' by done.
               pose proof Hp H' as Hp.
-              pose proof inflow_delete_outset_KT Jn n k (Cr !!! k) Jn'_temp as Hin'. 
-              assert (Jn'_temp = inflow_delete_KT Jn n k (Cr !!! k)) 
+              pose proof inflow_delete_inset_KT Jn n k (Cr !!! k) Jn_temp as Hin'. 
+              assert (Jn_temp = inflow_delete_KT Jn n k (Cr !!! k)) 
                     as HJn_t by done.  
               pose proof Hin' HJn_t n as [Hp' _].
               pose proof Hp' H' as Hp'.
               by rewrite Hp' in Hp. }
-              assert ((k',t') ∈ inset_KT Jn' n → 
+            assert ((k',t') ∈ inset_KT Jn' n → 
                        ((k',t') ∈ inset_KT Jn n) ∨ (k',t') = (k, T)) as Hkt'.
-              { intros Hin. rewrite Inset in Hin. set_solver. }
-              intros Hin. apply Hkt' in Hin.
-              destruct Hin as [Hin | Hin].
-              by pose proof Hφ3 k' t' Hin as Hφ3.
-              inversion Hin.
-              admit.
-          }  
+            { intros Hin. rewrite Inset in Hin. set_solver. }
+            intros Hin. apply Hkt' in Hin.
+            destruct Hin as [Hin | Hin].
+            by pose proof Hφ3 k' t' Hin as Hφ3.
+            inversion Hin.
+            by pose proof Hφ0 k. }  
           iMod "AU" as (t' H')"[MCS [_ Hclose]]".
           iAssert (⌜t' = T⌝)%I as %Ht'. 
           { iPoseProof ((auth_agree γ_te) with "[MCS_auth] [MCS]") as "%".
@@ -1149,10 +1341,10 @@ Section multicopy.
           iCombine "MCS◯t MCS◯h" as "MCS".
           iCombine "MCS●t MCS●h" as "MCS_auth".
           iMod ("Hclose" with "MCS") as "HΦ".            
-          
-          
+            
+            
           iModIntro.
-          iSplitR "HΦ node_n HnP_t HnP_C HnP_frac".
+          iSplitR "HΦ node_r HnP_t HnP_C HnP_frac".
           { iNext. iExists (T+1), (H1 ∪ {[(k, T)]}), I1, J1, R1.
             iFrame "∗ %".   
             rewrite (big_sepS_delete _ (domm I1) r); last by eauto.
@@ -1168,165 +1360,408 @@ Section multicopy.
               iFrame "∗#". assert (n =? r = false) as Hnr. 
               { by rewrite beq_nat_false_iff. } 
               by rewrite Hnr. }
-            iApply (big_opS_proper (λ y, ∃ (bn0 : bool) (Cn0 Bn0 : gmap K natUR),
+            iApply (big_sepS_mono (λ y, ∃ (bn0 : bool) (Cn0 Bn0 : gmap K natUR),
                                       lockLoc y ↦ #bn0
                                     ∗ (if bn0 then True else
                                        nodePred γ_e γ_c γ_b γ_t γ_s r y Cn0 Bn0)
                                     ∗ nodeShared γ_I γ_J γ_R γ_e γ_c γ_b γ_f γ_cir
-                                              r y Cn0 Bn0 H1 )%I
+                                              r y Cn0 Bn0 T H1 )%I
                                    (λ y, ∃ (bn0 : bool) (Cn0 Bn0 : gmap K natUR),
                                       lockLoc y ↦ #bn0
                                     ∗ (if bn0 then True else
                                        nodePred γ_e γ_c γ_b γ_t γ_s r y Cn0 Bn0)
                                     ∗ nodeShared γ_I γ_J γ_R γ_e γ_c γ_b γ_f γ_cir
-                                              r y Cn0 Bn0 (H1 ∪ {[(k, T)]}) )%I
+                                              r y Cn0 Bn0 (T+1) (H1 ∪ {[(k, T)]}) )%I
                                    (domm I1 ∖ {[r]} ∖ {[n]})); try done.
-            intros y y_dom. assert (y ≠ r) as Hy by set_solver. iFrame. iSplit;
-            iIntros "Hstar"; iDestruct "Hstar" as (b C B)"(Hl & Hlif & HnS)";
-            iExists b, C, B; iFrame; 
+            intros y y_dom. assert (y ≠ r) as Hy by set_solver. iFrame.
+            iIntros "Hstar". iDestruct "Hstar" as (b C B)"(Hl & Hlif & HnS)".
+            iExists b, C, B. iFrame. 
             iDestruct "HnS" as (esy Iy Jy Ry)"(HnS_frac & HnS_si & HnS_FP 
-                          & HnS_cl & HnS_oc & HnS_if & HnS_star & Hφ)";
-            iExists esy, Iy, Jy, Ry; iFrame; 
-            assert (y =? r = false) as Hyr by (rewrite beq_nat_false_iff; done);
-            iEval (rewrite Hyr); done. } 
+                          & HnS_cl & HnS_oc & HnS_if & HnS_star & Hφ0 & Hφ)".
+            iExists esy, Iy, Jy, Ry. iFrame.
+            iDestruct "Hφ0" as %Hφ0. 
+            assert (y =? r = false) as Hyr by (rewrite beq_nat_false_iff; done).
+            iEval (rewrite Hyr). iPureIntro. split; try done.
+            intros k'. pose proof Hφ0 k'. 
+            apply (Nat.le_trans _ T _); try done. lia. } 
           wp_pures.  
-          awp_apply (unlockNode_spec_high with "[] [] [HnP_t HnP_C HnP_frac node_n]")
+          awp_apply (unlockNode_spec_high with "[] [] [HnP_t HnP_C HnP_frac node_r]")
                 without "HΦ"; try done. iExists es, (T + 1). iFrame.
                 by iEval (rewrite <-beq_nat_refl).
           iAaccIntro with ""; try eauto with iFrame.
-          
-          
-          
-        * iAssert (outflow_constraints r Ir Jr Rr es Cr' Br')%I 
-                    with "[HnS_oc]" as "HnS_oc".
-          { admit. }
-          iAssert (φ1 Br' Cr' Ir ∗ φ2 r Br' Ir ∗ φ3 r Br' Jr ∗ φ4 r Br' Rr 
-                  ∗ φ5 r Rr)%I with "[Hφ]" as "Hφ".
-          { admit. }  
-          iMod "AU" as (t' H')"[MCS [_ Hclose]]".
-          iAssert (⌜t' = T⌝)%I as %Ht'. { admit. } replace t'.
-          iAssert (⌜H' = H1⌝)%I as %H1'. { admit. } replace H'.
-          iAssert (MCS γ_te γ_he (T+1) (H1 ∪ {[(k, T)]}) ∗
-                   MCS_auth γ_te γ_he (T+1) (H1 ∪ {[(k, T)]}))%I
-            with "[MCS MCS_auth]" as "(MCS & MCS_auth)".
-          { admit. }
-          iMod ("Hclose" with "MCS") as "HΦ".            
-                    
-          
-          
-          iModIntro.
-          iSplitR "HΦ node_n HnP_t HnP_C HnP_frac".
-          { iNext. iExists (T+1), (H1 ∪ {[(k, T)]}), I1, J1, R1.
-            iFrame.   
-            rewrite (big_sepS_delete _ (domm I1) r); last by eauto.
-            iSplitL "Hl_r Hlif_r HnS_cl HnS_star Hφ HnS_frac HnS_oc HnS_si HnS_if".
-            { iExists true, Cr', Br'. iFrame.
-              unfold nodeShared. iExists es, Ir, Jr, Rr.
-              iFrame "∗#". iEval (rewrite <-beq_nat_refl) in "HnS_if".
-              iDestruct "HnS_if" as "(_ & HnS_if)".
-              iEval (rewrite <-beq_nat_refl). iFrame "%∗". }        
-            iApply (big_opS_proper (λ y, ∃ (bn0 : bool) (Cn0 Bn0 : gmap K natUR),
-                                      lockLoc y ↦ #bn0
-                                    ∗ (if bn0 then True else
-                                       nodePred γ_e γ_c γ_b γ_t γ_s r y Cn0 Bn0)
-                                    ∗ nodeShared γ_I γ_J γ_R γ_e γ_c γ_b γ_f γ_cir
-                                              r y Cn0 Bn0 H1 )%I
-                                   (λ y, ∃ (bn0 : bool) (Cn0 Bn0 : gmap K natUR),
-                                      lockLoc y ↦ #bn0
-                                    ∗ (if bn0 then True else
-                                       nodePred γ_e γ_c γ_b γ_t γ_s r y Cn0 Bn0)
-                                    ∗ nodeShared γ_I γ_J γ_R γ_e γ_c γ_b γ_f γ_cir
-                                              r y Cn0 Bn0 (H1 ∪ {[(k, T)]}) )%I
-                                   (domm I1 ∖ {[r]})); try done.
-            intros y y_dom. assert (y ≠ r) as Hy by set_solver. iFrame. iSplit;
-            iIntros "Hstar"; iDestruct "Hstar" as (b C B)"(Hl & Hlif & HnS)";
-            iExists b, C, B; iFrame; 
-            iDestruct "HnS" as (esy Iy Jy Ry)"(HnS_frac & HnS_si & HnS_FP 
-                          & HnS_cl & HnS_oc & HnS_if & HnS_star & Hφ)";
-            iExists esy, Iy, Jy, Ry; iFrame; 
-            assert (y =? r = false) as Hyr by (rewrite beq_nat_false_iff; done);
-            iEval (rewrite Hyr); done. } 
-          wp_pures.  
-          awp_apply (unlockNode_spec_high with "[] [] [HnP_t HnP_C HnP_frac node_n]")
-                without "HΦ"; try done. iExists es, (T + 1). iFrame.
-                by iEval (rewrite <-beq_nat_refl).
-          iAaccIntro with ""; try eauto with iFrame.
-      + intros Cr_k.
-        set (Br' := <[k := T]>Br).
-        iAssert (⌜Br' = map_of_set (H1 ∪ {[(k, T)]})⌝)%I as %Br_eq_H1.
-        { admit. }
-        iAssert ([∗ set] k0 ∈ KS, own (γ_cir r k0) 
-                    (● {| max_nat_car := Br' !!! k0 |}))%I 
-            with "[HnS_star]" as "HnS_star".
-        { admit. }     
-        iAssert (frac_ghost_state γ_e γ_c γ_b r es Cr' Br' ∗ 
-                    frac_ghost_state γ_e γ_c γ_b r es Cr' Br')%I 
-              with "[HnP_frac HnS_frac]" as "(HnP_frac & HnS_frac)".
-        { admit. }
-        assert ((∃ n, k ∈ es !!! n ∧ n ≠ r) ∨ (∀ n, k ∉ es !!! n)) as Hes.
-        { admit. } destruct Hes as [Hes | Hes].
-        * destruct Hes as [n [k_in_es n_neq_r]].
-          set (Jr'_out_r := (nzmap_imerge 
-             (λ k' a1 _, if (decide (k' = (k, T))) then 1 else a1)
-                         (out Jr n) (∅)): (KT_multiset)).
-          set (Jr'_out := (nzmap_imerge 
-                      (λ k' a1 _, if (decide (k = r)) then Jr'_out_r else a1)
-                      (out_map Jr) (∅)) : (nzmap Node KT_multiset)).
-          set (Jr1' := ({| infR := inf_map Jr ; outR := Jr'_out |})).
-          set (Jr' := ∅: (KT_flowint_ur K)).
-          set (Ir' := ∅: (KT_flowint_ur K)).
+        * iEval (rewrite (big_sepS_delete (_) (KS) k); last by eauto) in "HnS_star".
+          iDestruct "HnS_star" as "(Hk & HnS_star')".
+          iAssert (⌜Br !!! k ≤ T⌝)%I as %Br_le_T. 
+          { iDestruct "Hφ" as "(% & _)".
+            iPureIntro. rename H into H'.
+            by pose proof H' k. }
+          iMod (own_update (γ_cir r k) (● (MaxNat (Br !!! k))) 
+                    (● (MaxNat (Br' !!! k))) with "Hk") as "Hk".
+          { apply (auth_update_auth _ _ (MaxNat (Br' !!! k))).
+            apply max_nat_local_update.
+            simpl. rewrite HBr'.
+            by rewrite lookup_total_insert. }        
+          iAssert ([∗ set] k0 ∈ KS, own (γ_cir r k0) 
+                      (● {| max_nat_car := Br' !!! k0 |}))%I 
+              with "[HnS_star' Hk]" as "HnS_star".
+          { iEval (rewrite (big_sepS_delete (_) (KS) k); last by eauto).
+            iFrame "Hk".        
+            iApply (big_opS_proper 
+                 (λ y, own (γ_cir r y) (● {| max_nat_car := Br' !!! y |}))
+                 (λ y, own (γ_cir r y) (● {| max_nat_car := Br !!! y |})) 
+                 (KS ∖ {[k]})).
+            intros x Hx. assert (x ≠ k) as H' by set_solver.
+            iFrame. iSplit. 
+            iIntros "H". iEval (rewrite HBr') in "H".
+            assert (<[k:=T]> Br !!! x = Br !!! x) as H''. 
+            { apply lookup_total_insert_ne; try done. } 
+            by iEval (rewrite H'') in "H".       
+            iIntros "H". iEval (rewrite HBr').
+            assert (<[k:=T]> Br !!! x = Br !!! x) as H''. 
+            { apply lookup_total_insert_ne; try done. } 
+            by iEval (rewrite H'').
+            done. }
+          iMod ((frac_update γ_e γ_c γ_b r es Cr Br es Cr' Br') 
+                      with "[$HnP_frac $HnS_frac]") as "(HnP_frac & HnS_frac)".
+          set (Ir' := outflow_delete_KT Ir n k (Br !!! k)).
+          set (Jr' := outflow_insert_KT Jr n k T).
+          iPoseProof (node_edgeset_disjoint with "node_r") as "%".
+          rename H into Disj_es. 
           iAssert (outflow_constraints r Ir' Jr' Rr es Cr' Br')%I 
                     with "[HnS_oc]" as "HnS_oc".
-          { admit. }
+          { iDestruct "HnS_oc" as "(% & % & %)".
+            rename H into OC_1. rename H2 into OC_2.
+            rename H3 into OC_3.
+            iPureIntro. split; last split; try done.
+            - intros n' k' t'.
+              destruct (decide (n' = n)).
+              + assert (outset_KT Ir' n = (outset_KT Ir n) ∖ {[(k, Br !!! k)]}) 
+                                                                   as Out_eq.
+                { pose proof outflow_delete_outset_KT Ir n k (Br !!! k) Ir' as H'. 
+                  assert (Ir' = outflow_delete_KT Ir n k (Br !!! k)) as HIr' by done.
+                  pose proof H' HIr' n as [Hout _].
+                  assert (n = n) as Hn by done.
+                  by pose proof Hout Hn. }
+                replace n'. split.
+                * intros Hout.
+                  assert ((k', t') ∈ outset_KT Ir n) as Hkt'.
+                  { clear -Out_eq Hout. set_solver. }
+                  apply OC_1 in Hkt'.
+                  destruct (decide (k' = k)).
+                  rewrite e0 in Hout.
+                  destruct Hkt' as [_ [_ Hkt']].
+                  rewrite e0 in Hkt'.
+                  rewrite <-Hkt' in Hout.
+                  clear -Hout Out_eq.
+                  set_solver.
+                  replace Cr'.
+                  rewrite lookup_total_insert_ne; try done.
+                  rewrite HBr'.
+                  rewrite lookup_total_insert_ne; try done.
+                * intros Hout.
+                  destruct (decide (k' = k)).
+                  destruct Hout as [_ [Hout _]].
+                  rewrite e0 in Hout.
+                  replace Cr' in Hout.
+                  rewrite lookup_total_insert in Hout.
+                  destruct Max_tsH1 as [_ H']. lia.
+                  replace Cr' in Hout.
+                  rewrite lookup_total_insert_ne in Hout; try done.
+                  rewrite HBr' in Hout.
+                  rewrite lookup_total_insert_ne in Hout; try done.
+                  apply OC_1 in Hout.
+                  clear -Hout Out_eq n0. set_solver.
+              + assert (outset_KT Ir' n' = outset_KT Ir n') as Out_eq.
+                { pose proof outflow_delete_outset_KT Ir n k (Br !!! k) Ir' as H'. 
+                  assert (Ir' = outflow_delete_KT Ir n k (Br !!! k)) as HIr' by done.
+                  pose proof H' HIr' n' as [_ Hout].
+                  by pose proof Hout n0. }
+                rewrite Out_eq.
+                split.
+                * intros Hout.
+                  apply OC_1 in Hout.
+                  destruct (decide (k' = k)).
+                  destruct Hout as [H' _].
+                  rewrite e in H'.
+                  pose proof Disj_es n' n n0 as H''.
+                  clear -H'' H' k_in_es. 
+                  set_solver.
+                  replace Cr'.
+                  rewrite lookup_total_insert_ne; try done.
+                  rewrite HBr'.
+                  rewrite lookup_total_insert_ne; try done.
+                * intros Hout.
+                  destruct (decide (k' = k)).
+                  destruct Hout as [H' _].
+                  rewrite e in H'.
+                  pose proof Disj_es n' n n0 as H''.
+                  clear -H'' H' k_in_es. 
+                  set_solver.
+                  replace Cr' in Hout.
+                  rewrite lookup_total_insert_ne in Hout; try done.
+                  rewrite HBr' in Hout.
+                  rewrite lookup_total_insert_ne in Hout; try done.
+                  by apply OC_1 in Hout.
+            - intros n' k' t'.
+              destruct (decide (n' = n)).
+              + assert (outset_KT Jr' n = outset_KT Jr n ∪ {[k, T]}) as Outset.
+                { pose proof outflow_insert_outset_KT Jr n k T Jr' as Houts.
+                  assert (Jr' = outflow_insert_KT Jr n k T) as HJr' by done.
+                  pose proof Houts HJr' n' as [Hp _].
+                  pose proof Hp e as Hp.
+                  by rewrite <-e. }
+                replace n'.  
+                assert ((k',t') ∈ outset_KT Jr' n → 
+                       ((k',t') ∈ outset_KT Jr n) ∨ (k',t') = (k, T)) as Hkt'.
+                { intros Hout. rewrite Outset in Hout.
+                  set_solver. }
+                split.
+                * intros Hout. pose proof Hkt' Hout as Hkt'.
+                  destruct Hkt' as [Hkt' | Hkt'].
+                  ** apply OC_2 in Hkt'.
+                     destruct Hkt' as [Hkt'_1 [Hkt'_2 Hkt'_3]]. 
+                     split; try done.
+                     destruct (decide (k' = k)).
+                     rewrite e0 in Hkt'_3.
+                     clear -Cr_k Hkt'_3. lia.
+                     replace Cr'. 
+                     rewrite lookup_total_insert_ne; try done.
+                  ** inversion Hkt'.
+                     repeat split; try done.
+                     replace Cr'.
+                     rewrite lookup_total_insert; try done.
+                     replace Cr'.
+                     rewrite lookup_total_insert; try done.
+                     by destruct Max_tsH1 as [_ H'].
+                * intros [Hk1 [Hk2 Hk3]].
+                  destruct (decide (k' = k)).
+                  ** replace k'.
+                     rewrite e0 in Hk1.
+                     rewrite e0 in Hk2.
+                     replace Cr' in Hk2. 
+                     rewrite lookup_total_insert in Hk2.
+                     replace t'. rewrite Outset.
+                     set_solver.
+                  ** replace Cr' in Hk2.
+                     rewrite lookup_total_insert_ne in Hk2; try done.
+                     replace Cr' in Hk3.
+                     rewrite lookup_total_insert_ne in Hk3; try done.
+                     assert (k' ∈ es !!! n ∧ Cr !!! k' = t' ∧ Cr !!! k' > 0) 
+                                        as Hkt; try done.
+                     apply OC_2 in Hkt.
+                     rewrite Outset.
+                     clear -Hkt n0. set_solver.
+              + assert (outset_KT Jr' n' = outset_KT Jr n') as Outset.
+                { pose proof outflow_insert_outset_KT Jr n k T Jr' as Houts.
+                  assert (Jr' = outflow_insert_KT Jr n k T) as HJr' by done.
+                  pose proof Houts HJr' n' as [_ Hp].
+                  by pose proof Hp n0 as Hp. }
+                rewrite Outset.
+                split.
+                * intros Hout.
+                  apply OC_2 in Hout.
+                  destruct Hout as [Hout1 [Hout2 Hout3]].
+                  split; try done.
+                  destruct (decide (k' = k)).
+                  ** rewrite e in Hout1.
+                     pose proof Disj_es n' n n0 as H'.
+                     clear -H' Hout1 k_in_es. 
+                     set_solver.
+                  ** replace Cr'.
+                     rewrite lookup_total_insert_ne; try done.
+                * intros [Hout1 [Hout2 Hout3]].
+                  destruct (decide (k' = k)).
+                  ** rewrite e in Hout1.
+                     pose proof Disj_es n' n n0 as H'.
+                     clear -H' Hout1 k_in_es. 
+                     set_solver.
+                  ** replace Cr' in Hout2.
+                     rewrite lookup_total_insert_ne in Hout2; try done.
+                     replace Cr' in Hout3.
+                     rewrite lookup_total_insert_ne in Hout3; try done.
+                     apply OC_2.
+                     split; try done. }  
           iAssert (inFP γ_f n)%I as "#FP_n". 
           { iApply "HnS_cl". iPureIntro.
             clear -k_in_es. set_solver. }
           iAssert (⌜n ∈ domm I1⌝)%I as %n_in_I.
-          { admit. }
+          { by iPoseProof (inFP_domm _ _ _ with "[$FP_n] [$Hf]") as "H'". }
           rewrite (big_sepS_delete _ (domm I1 ∖ {[r]}) n); last by set_solver.
           iDestruct "Hstar'" as "(H_n & Hstar')".
           iDestruct "H_n" as (bn Cn Bn)"(Hl_n & Hlif_n & HnS_n)".
           iDestruct "HnS_n" as (es_n In Jn Rn) 
             "(HnS_fracn & HnS_sin & HnS_FPn & HnS_cln & HnS_ocn & 
                                         HnS_ifn & HnS_starn & Hφn)".
-          set (Jn' := ∅: (KT_flowint_ur K)).
-          set (In' := ∅: (KT_flowint_ur K)).
+          set (In' := inflow_delete_KT In n k (Br !!! k)).
+          set (Jn' := inflow_insert_KT Jn n k T).
           iAssert (singleton_interfaces_ghost_state γ_I γ_J γ_R r Ir' Jr' Rr
             ∗ singleton_interfaces_ghost_state γ_I γ_J γ_R n In' Jn' Rn)%I 
                     with "[HnS_si HnS_sin]" as "(HnS_si & HnS_sin)".
-          { admit. }          
+          { unfold singleton_interfaces_ghost_state. 
+            iDestruct "HnS_si" as "(HrI & HrJ & HrR & Domm_rI & Domm_rJ & Domm_rR)".
+            iDestruct "HnS_sin" as "(HnI & HnJ & HnR & Domm_nI & Domm_nJ & Domm_nR)".
+            assert (domm Jn' = domm Jn) as H'.
+            { assert (Jn' = inflow_insert_KT Jn n k T) as HJn' by done.
+              apply (inflow_insert_domm _ n k T); try done. }
+            assert (domm In' = domm In) as H''.
+            { assert (In' = inflow_delete_KT In n k (Br !!! k)) as HJn' by done.
+              apply (inflow_delete_domm _ n k (Br !!! k)); try done. }
+            rewrite H' H''. iFrame.
+            destruct H' as []. destruct H'' as [].
+            iCombine "HrJ HnJ" as "HrnJ".
+            iCombine "HrI HnI" as "HrnI".
+            assert (Jr ⋅ Jn = Jr' ⋅ Jn') as H'.
+            { apply (flow_insert_eq_KT Jr Jr' _ _ n k T);
+                         try done. }
+            assert (Ir ⋅ In = Ir' ⋅ In') as H''.
+            { apply (flow_delete_eq_KT Ir Ir' _ _ n k (Br !!! k));
+                         try done. }
+            rewrite H' H''.
+            iEval (rewrite auth_frag_op) in "HrnJ".
+            iEval (rewrite auth_frag_op) in "HrnI".
+            iDestruct "HrnJ" as "(HrJ & HnJ)".
+            iDestruct "HrnI" as "(HrI & HnI)". iFrame. }
           iAssert (outflow_constraints n In' Jn' Rn es_n Cn Bn)%I
             with "[HnS_ocn]" as "HnS_ocn".
-          { admit. }
-          iAssert (φ1 Br' Cr' Ir' ∗ φ2 r Br' Ir' ∗ φ3 r Br' Jr' ∗ φ4 r Br' Rr 
-                  ∗ φ5 r Rr)%I with "[Hφ]" as "Hφ".
-          { admit. }  
-          iAssert (φ1 Bn Cn In' ∗ φ2 n Bn In' ∗ φ3 n Bn Jn' ∗ φ4 n Bn Rn 
-                  ∗ φ5 n Rn)%I with "[Hφn]" as "Hφn".
-          { admit. }  
+          { iDestruct "HnS_ocn" as "(% & % & %)".
+            rename H into OC_1. rename H2 into OC_2.
+            rename H3 into OC_3. 
+            iPureIntro. split; last split; try done. }
+          iDestruct "Inf_R" as %Inf_R.
+          iPoseProof ((auth_own_incl γ_R R1 Rr) with "[HR HnS_si]")
+              as (Ro) "%". 
+          { unfold singleton_interfaces_ghost_state.
+            iDestruct "HnS_si" as "(_ & _ & H' & _)". 
+            iFrame. } rename H into Incl_R1.
+          iPoseProof (own_valid with "HR") as "%".
+          rename H into Valid_R1.
+          iAssert (⌜domm Rr = {[r]}⌝)%I as "%".
+          { by iDestruct "HnS_si" as "(_&_&_&_&_&H')". }
+          rename H into Domm_Rr.
+          iAssert (⌜φ0 Br' (T+1)⌝ ∗ ⌜φ1 Br' Cr' Ir'⌝ ∗ ⌜φ2 r Br' Ir'⌝ ∗ ⌜φ3 r Br' Jr'⌝ 
+                  ∗ ⌜φ4 r Br' Rr⌝ ∗ ⌜φ5 r Rr⌝)%I with "[Hφ]" as "Hφ".
+          { iDestruct "Hφ" as %Hφ. 
+            destruct Hφ as [Hφ0 [Hφ1 [Hφ2 [Hφ3 [Hφ4 Hφ5]]]]].
+            iPureIntro. repeat split; try done.
+            - intros k'. destruct (decide (k' = k)).
+              rewrite HBr'. rewrite e. rewrite lookup_total_insert. lia.
+              rewrite HBr'. rewrite lookup_total_insert_ne; try done.
+              pose proof Hφ0 k' as H'. clear -H'. Search (≤). 
+              apply (Nat.le_trans _ T _); try done. lia. 
+            - intros k'.
+              destruct (decide (k' = k)).
+              right. replace Cr'. rewrite HBr'.
+              replace k'.
+              rewrite lookup_total_insert.
+              by rewrite lookup_total_insert.
+              pose proof Hφ1 k' as Hφ1.
+              destruct Hφ1 as [Hφ1 | Hφ1].
+              destruct Hφ1 as [t' [n' Hφ1]].
+              destruct (decide (n' = n)).
+              assert (outset_KT Ir' n' = (outset_KT Ir n') ∖ {[(k, Br !!! k)]}) 
+                                                                as Out_eq.
+              { pose proof outflow_delete_outset_KT Ir n k (Br !!! k) Ir' as H'. 
+                assert (Ir' = outflow_delete_KT Ir n k (Br !!! k)) as HIr' by done.
+                pose proof H' HIr' n' as [Hout _].
+                by pose proof Hout e. }
+              rewrite e in Out_eq. rewrite e in Hφ1.
+              left. exists t', n.
+              clear -n0 Out_eq Hφ1. set_solver.
+              assert (outset_KT Ir' n' = outset_KT Ir n') as Out_eq.
+              { pose proof outflow_delete_outset_KT Ir n k (Br !!! k) Ir' as H'. 
+                assert (Ir' = outflow_delete_KT Ir n k (Br !!! k)) as HIr' by done.
+                pose proof H' HIr' n' as [_ Hout].
+                by pose proof Hout n1. }
+              rewrite <-Out_eq in Hφ1.
+              left. exists t', n'. done.    
+              right. rewrite HBr'.
+              rewrite lookup_total_insert_ne; try done.
+              replace Cr'.
+              rewrite lookup_total_insert_ne; try done.
+            - intros k' t' Hins.
+              pose proof Infz_rI r as Infz_rI.
+              assert (Ir' = outflow_delete_KT Ir n k (Br !!! k)) as H' by done.
+              pose proof outflow_delete_inf_eq_KT Ir n k (Br !!! k) Ir' H' r as H''.
+              rewrite <-H'' in Infz_rI.
+              rewrite Infz_rI in Hins.
+              exfalso. clear -Hins. set_solver.
+            - intros k' t' Hins.
+              pose proof Infz_rJ r as Infz_rJ.
+              assert (inset_KT Jr' r = inset_KT Jr r) as H'.
+              { assert (inset_KT Jr' r = inset_KT Jr r) as H''.
+                apply (outflow_insert_inf_eq_KT _ n k T); try done.
+                done. }
+              rewrite H' in Hins. rewrite Infz_rJ in Hins.
+              exfalso. clear -Hins. set_solver.
+            - intros k'. right.
+              apply (inset_monotone R1 Rr Ro); try done.
+              by rewrite <-auth_auth_valid.
+              pose proof Inf_R r k' as Inf_R.
+              by rewrite <-beq_nat_refl in Inf_R.
+              rewrite Domm_Rr. clear. set_solver. } 
+          iAssert (⌜φ0 Bn (T+1)⌝ ∗ ⌜φ1 Bn Cn In'⌝ ∗ ⌜φ2 n Bn In'⌝ ∗ ⌜φ3 n Bn Jn'⌝ 
+                  ∗ ⌜φ4 n Bn Rn⌝ ∗ ⌜φ5 n Rn⌝)%I with "[Hφn]" as "Hφn".
+          { iDestruct "Hφn" as %Hφ. 
+            destruct Hφ as [Hφ0 [Hφ1 [Hφ2 [Hφ3 [Hφ4 Hφ5]]]]].
+            iPureIntro. repeat split; try done.
+            - intros k'. pose proof Hφ0 k' as H'.
+              apply (Nat.le_trans _ T _); try done. lia. 
+            - intros k' t'. 
+              assert (inset_KT In' n = inset_KT In n ∖ {[k, Br !!! k]}) as Inset.
+              { pose proof inflow_delete_inset_KT In n k (Br !!! k) In' as Hin.
+                assert (In' = inflow_delete_KT In n k (Br !!! k)) as HIn' by done.
+                pose proof Hin HIn' n as [Hp _].
+                assert (n = n) as H' by done.
+                by pose proof Hp H' as Hp. }
+              intros Hin. 
+              assert ((k', t') ∈ inset_KT In n) as H'.
+              { clear -Hin Inset. set_solver. } 
+              by pose proof Hφ2 k' t' H' as Hφ2.
+            - intros k' t'. 
+              assert (inset_KT Jn' n = inset_KT Jn n ∪ {[k, T]}) as Inset.
+              { pose proof inflow_insert_inset_KT Jn n k T Jn' as Hin.
+                assert (Jn' = inflow_insert_KT Jn n k T) as HJn' by done.
+                pose proof Hin HJn' n as [Hp _].
+                assert (n = n) as H' by done.
+                by pose proof Hp H'. }
+              assert ((k',t') ∈ inset_KT Jn' n → 
+                         ((k',t') ∈ inset_KT Jn n) ∨ (k',t') = (k, T)) as Hkt'.
+              { intros Hin. rewrite Inset in Hin. set_solver. }
+              intros Hin. apply Hkt' in Hin.
+              destruct Hin as [Hin | Hin].
+              by pose proof Hφ3 k' t' Hin as Hφ3.
+              inversion Hin.
+              by pose proof Hφ0 k. }  
           iMod "AU" as (t' H')"[MCS [_ Hclose]]".
-          iAssert (⌜t' = T⌝)%I as %Ht'. { admit. } replace t'.
-          iAssert (⌜H' = H1⌝)%I as %H1'. { admit. } replace H'.
-          iAssert (MCS γ_te γ_he (T+1) (H1 ∪ {[(k, T)]}) ∗
-                   MCS_auth γ_te γ_he (T+1) (H1 ∪ {[(k, T)]}))%I
-            with "[MCS MCS_auth]" as "(MCS & MCS_auth)".
-          { admit. }
+          iAssert (⌜t' = T⌝)%I as %Ht'. 
+          { iPoseProof ((auth_agree γ_te) with "[MCS_auth] [MCS]") as "%".
+            unfold MCS_auth. by iDestruct "MCS_auth" as "(H' & _)".
+            by iDestruct "MCS" as "(H' & _)".
+            by iPureIntro. } replace t'.
+          iAssert (⌜H' = H1⌝)%I as %H1'.
+          { iPoseProof ((auth_agree' γ_he) with "[MCS_auth] [MCS]") as "%".
+            unfold MCS_auth. by iDestruct "MCS_auth" as "(_ & H'')".
+            by iDestruct "MCS" as "(_ & H')".
+            by iPureIntro. } replace H'.
+          iDestruct "MCS" as "(MCS◯t & MCS◯h)".
+          iDestruct "MCS_auth" as "(MCS●t & MCS●h)".
+          iMod ((auth_update γ_te (T+1) T T) with "MCS●t MCS◯t") 
+                                              as "(MCS●t & MCS◯t)".
+          iMod ((auth_update' γ_he (H1 ∪ {[(k, T)]}) H1 H1) with "MCS●h MCS◯h") 
+                                              as "(MCS●h & MCS◯h)".
+          iCombine "MCS◯t MCS◯h" as "MCS".
+          iCombine "MCS●t MCS●h" as "MCS_auth".
           iMod ("Hclose" with "MCS") as "HΦ".            
-                    
-          
-          
           iModIntro.
-          iSplitR "HΦ node_n HnP_t HnP_C HnP_frac".
+          iSplitR "HΦ node_r HnP_t HnP_C HnP_frac".
           { iNext. iExists (T+1), (H1 ∪ {[(k, T)]}), I1, J1, R1.
-            iFrame.   
+            iFrame "∗%".   
             rewrite (big_sepS_delete _ (domm I1) r); last by eauto.
-            iSplitL "Hl_r Hlif_r HnS_cl HnS_star Hφ HnS_frac HnS_oc HnS_si HnS_if".
+            iSplitL "Hl_r Hlif_r HnS_cl HnS_star Hφ HnS_frac HnS_oc HnS_si".
             { iExists true, Cr', Br'. iFrame.
               unfold nodeShared. iExists es, Ir', Jr', Rr.
-              iFrame "∗#". iEval (rewrite <-beq_nat_refl) in "HnS_if".
-              iDestruct "HnS_if" as "(_ & HnS_if)".
-              iEval (rewrite <-beq_nat_refl). iFrame "%∗".
-              unfold inflow_zero. admit. }        
+              iFrame "∗#".
+              iEval (rewrite <-beq_nat_refl). iFrame "%∗". }        
             rewrite (big_sepS_delete _ (domm I1 ∖ {[r]}) n); last by set_solver.
             iSplitL "Hl_n Hlif_n HnS_cln HnS_starn Hφn HnS_fracn HnS_ocn 
                         HnS_sin HnS_ifn".
@@ -1334,34 +1769,233 @@ Section multicopy.
               iFrame "∗#". assert (n =? r = false) as Hnr. 
               { by rewrite beq_nat_false_iff. } 
               by rewrite Hnr. }
-            iApply (big_opS_proper (λ y, ∃ (bn0 : bool) (Cn0 Bn0 : gmap K natUR),
+            iApply (big_sepS_mono (λ y, ∃ (bn0 : bool) (Cn0 Bn0 : gmap K natUR),
                                       lockLoc y ↦ #bn0
                                     ∗ (if bn0 then True else
                                        nodePred γ_e γ_c γ_b γ_t γ_s r y Cn0 Bn0)
                                     ∗ nodeShared γ_I γ_J γ_R γ_e γ_c γ_b γ_f γ_cir
-                                              r y Cn0 Bn0 H1 )%I
+                                              r y Cn0 Bn0 T H1 )%I
                                    (λ y, ∃ (bn0 : bool) (Cn0 Bn0 : gmap K natUR),
                                       lockLoc y ↦ #bn0
                                     ∗ (if bn0 then True else
                                        nodePred γ_e γ_c γ_b γ_t γ_s r y Cn0 Bn0)
-                                    ∗ nodeShared γ_I γ_J γ_R γ_e γ_c γ_b γ_f γ_cir
-                                              r y Cn0 Bn0 (H1 ∪ {[(k, T)]}) )%I
+                                     ∗ nodeShared γ_I γ_J γ_R γ_e γ_c γ_b γ_f γ_cir
+                                              r y Cn0 Bn0 (T+1) (H1 ∪ {[(k, T)]}) )%I
                                    (domm I1 ∖ {[r]} ∖ {[n]})); try done.
-            intros y y_dom. assert (y ≠ r) as Hy by set_solver. iFrame. iSplit;
-            iIntros "Hstar"; iDestruct "Hstar" as (b C B)"(Hl & Hlif & HnS)";
-            iExists b, C, B; iFrame; 
+            intros y y_dom. assert (y ≠ r) as Hy by set_solver. iFrame.
+            iIntros "Hstar". iDestruct "Hstar" as (b C B)"(Hl & Hlif & HnS)".
+            iExists b, C, B; iFrame. 
             iDestruct "HnS" as (esy Iy Jy Ry)"(HnS_frac & HnS_si & HnS_FP 
-                          & HnS_cl & HnS_oc & HnS_if & HnS_star & Hφ)";
-            iExists esy, Iy, Jy, Ry; iFrame; 
+                        & HnS_cl & HnS_oc & HnS_if & HnS_star & Hφ0 & Hφ)".
+            iExists esy, Iy, Jy, Ry; iFrame. 
+            assert (y =? r = false) as Hyr by (rewrite beq_nat_false_iff; done).
+            iEval (rewrite Hyr).
+            iDestruct "Hφ0" as %Hφ0. iPureIntro; split; try done.
+            intros k'; pose proof Hφ0 k' as Hφ0.
+            apply (Nat.le_trans _ T _); try done. lia. } 
+            wp_pures.  
+            awp_apply (unlockNode_spec_high 
+                  with "[] [] [HnP_t HnP_C HnP_frac node_r]")
+                  without "HΦ"; try done. iExists es, (T + 1). iFrame.
+                  by iEval (rewrite <-beq_nat_refl).
+            iAaccIntro with ""; try eauto with iFrame.
+        + pose proof (out_edgeset_false k es Hes) as H'.
+          clear Hes. rename H' into Hes.
+          iMod ((frac_update γ_e γ_c γ_b r es Cr Br es Cr' Br') 
+               with "[$HnP_frac $HnS_frac]") as "(HnP_frac & HnS_frac)".
+          iAssert (⌜Br !!! k ≤ T⌝)%I as %Br_le_T. 
+          { iDestruct "Hφ" as "(% & _)".
+            iPureIntro. rename H into H'.
+            by pose proof H' k. }
+          iEval (rewrite (big_sepS_delete (_) (KS) k); last by eauto) in "HnS_star".
+          iDestruct "HnS_star" as "(Hk & HnS_star')".          
+          iMod (own_update (γ_cir r k) (● (MaxNat (Br !!! k))) 
+                    (● (MaxNat (Br' !!! k))) with "Hk") as "Hk".
+          { apply (auth_update_auth _ _ (MaxNat (Br' !!! k))).
+            apply max_nat_local_update.
+            simpl. rewrite HBr'.
+            by rewrite lookup_total_insert. }        
+          iAssert ([∗ set] k0 ∈ KS, own (γ_cir r k0) 
+                      (● {| max_nat_car := Br' !!! k0 |}))%I 
+              with "[HnS_star' Hk]" as "HnS_star".
+          { iEval (rewrite (big_sepS_delete (_) (KS) k); last by eauto).
+            iFrame "Hk".        
+            iApply (big_opS_proper 
+                 (λ y, own (γ_cir r y) (● {| max_nat_car := Br' !!! y |}))
+                 (λ y, own (γ_cir r y) (● {| max_nat_car := Br !!! y |})) 
+                 (KS ∖ {[k]})).
+            intros x Hx. assert (x ≠ k) as H' by set_solver.
+            iFrame. iSplit. 
+            iIntros "H". iEval (rewrite HBr') in "H".
+            assert (<[k:=T]> Br !!! x = Br !!! x) as H''. 
+            { apply lookup_total_insert_ne; try done. } 
+            by iEval (rewrite H'') in "H".       
+            iIntros "H". iEval (rewrite HBr').
+            assert (<[k:=T]> Br !!! x = Br !!! x) as H''. 
+            { apply lookup_total_insert_ne; try done. } 
+            by iEval (rewrite H'').
+            done. }
+          iAssert (outflow_constraints r Ir Jr Rr es Cr' Br')%I 
+                      with "[HnS_oc]" as "HnS_oc".
+          { iDestruct "HnS_oc" as "(% & % & %)".
+            rename H into OC_1. rename H2 into OC_2.
+            rename H3 into OC_3.
+            iPureIntro. split; last split; try done.
+            - intros n' k' t'. split.
+              + intros Hout.
+                pose proof OC_1 n' k' t' as [H' _].
+                apply H' in Hout.
+                destruct (decide (k' = k)).
+                * destruct Hout as [Hout _].
+                  rewrite e in Hout.
+                  pose proof Hes n' as Hes.
+                  clear - Hes Hout. set_solver.
+                * replace Cr'.
+                  rewrite lookup_total_insert_ne; try done.
+                  rewrite HBr'.
+                  rewrite lookup_total_insert_ne; try done.  
+              + intros Hout.
+                destruct (decide (k' = k)).
+                * destruct Hout as [Hout _].
+                  pose proof Hes n' as Hes.
+                  rewrite e in Hout.
+                  clear - Hes Hout. set_solver.
+                * replace Cr' in Hout.
+                  rewrite lookup_total_insert_ne in Hout; try done.
+                  rewrite HBr' in Hout.
+                  rewrite lookup_total_insert_ne in Hout; try done.
+                  by apply OC_1 in Hout.  
+            - intros n' k' t'. split.
+              + intros Hout.
+                pose proof OC_2 n' k' t' as [H' _].
+                apply H' in Hout.
+                destruct (decide (k' = k)).
+                * destruct Hout as [Hout _].
+                  rewrite e in Hout.
+                  pose proof Hes n' as Hes.
+                  clear - Hes Hout. set_solver.
+                * replace Cr'.
+                  rewrite lookup_total_insert_ne; try done.
+              + intros Hout.
+                destruct (decide (k' = k)).
+                * destruct Hout as [Hout _].
+                  pose proof Hes n' as Hes.
+                  rewrite e in Hout.
+                  clear - Hes Hout. set_solver.
+                * replace Cr' in Hout.
+                  rewrite lookup_total_insert_ne in Hout; try done.
+                  by apply OC_2 in Hout. }
+          iDestruct "Inf_R" as %Inf_R.
+          iPoseProof ((auth_own_incl γ_R R1 Rr) with "[HR HnS_si]")
+              as (Ro) "%". 
+          { unfold singleton_interfaces_ghost_state.
+            iDestruct "HnS_si" as "(_ & _ & H' & _)". 
+            iFrame. } rename H into Incl_R1.
+          iPoseProof (own_valid with "HR") as "%".
+          rename H into Valid_R1.
+          iAssert (⌜domm Rr = {[r]}⌝)%I as "%".
+          { by iDestruct "HnS_si" as "(_&_&_&_&_&H')". }
+          rename H into Domm_Rr.
+          iAssert (⌜φ0 Br' (T+1)⌝ ∗ ⌜φ1 Br' Cr' Ir⌝ ∗ ⌜φ2 r Br' Ir⌝ ∗ ⌜φ3 r Br' Jr⌝ 
+                  ∗ ⌜φ4 r Br' Rr⌝ ∗ ⌜φ5 r Rr⌝)%I with "[Hφ]" as "Hφ".
+          { iDestruct "Hφ" as %Hφ. 
+            destruct Hφ as [Hφ0 [Hφ1 [Hφ2 [Hφ3 [Hφ4 Hφ5]]]]].
+            iPureIntro. repeat split; try done.
+            - intros k'. destruct (decide (k' = k)).
+              rewrite HBr'. rewrite e. rewrite lookup_total_insert. lia.
+              rewrite HBr'. rewrite lookup_total_insert_ne; try done.
+              pose proof Hφ0 k' as H'. clear -H'. Search (≤). 
+              apply (Nat.le_trans _ T _); try done. lia. 
+            - intros k'. pose proof Hφ1 k' as H'.
+              destruct H' as [H' | H'].
+              by left.
+              destruct (decide (k' = k)).
+              right. replace k'.
+              rewrite lookup_total_insert.
+              replace Cr'.
+              by rewrite lookup_total_insert.
+              right.
+              rewrite lookup_total_insert_ne; try done.
+              replace Cr'.
+              rewrite lookup_total_insert_ne; try done.
+            - intros k' t' Hins.
+              pose proof Infz_rI r as Infz_rI.
+              rewrite Infz_rI in Hins.
+              exfalso. clear -Hins. set_solver.
+            - intros k' t' Hins.
+              pose proof Infz_rJ r as Infz_rJ.
+              rewrite Infz_rJ in Hins.
+              exfalso. clear -Hins. set_solver.
+            - intros k'. right.
+              apply (inset_monotone R1 Rr Ro); try done.
+              by rewrite <-auth_auth_valid.
+              pose proof Inf_R r k' as Inf_R.
+              by rewrite <-beq_nat_refl in Inf_R.
+              rewrite Domm_Rr. clear. set_solver. } 
+          iMod "AU" as (t' H')"[MCS [_ Hclose]]".
+          iAssert (⌜t' = T⌝)%I as %Ht'. 
+          { iPoseProof ((auth_agree γ_te) with "[MCS_auth] [MCS]") as "%".
+            unfold MCS_auth. by iDestruct "MCS_auth" as "(H' & _)".
+            by iDestruct "MCS" as "(H' & _)".
+            by iPureIntro. } replace t'.
+          iAssert (⌜H' = H1⌝)%I as %H1'.
+          { iPoseProof ((auth_agree' γ_he) with "[MCS_auth] [MCS]") as "%".
+            unfold MCS_auth. by iDestruct "MCS_auth" as "(_ & H'')".
+            by iDestruct "MCS" as "(_ & H')".
+            by iPureIntro. } replace H'.
+          iDestruct "MCS" as "(MCS◯t & MCS◯h)".
+          iDestruct "MCS_auth" as "(MCS●t & MCS●h)".
+          iMod ((auth_update γ_te (T+1) T T) with "MCS●t MCS◯t") 
+                                              as "(MCS●t & MCS◯t)".
+          iMod ((auth_update' γ_he (H1 ∪ {[(k, T)]}) H1 H1) with "MCS●h MCS◯h") 
+                                              as "(MCS●h & MCS◯h)".
+          iCombine "MCS◯t MCS◯h" as "MCS".
+          iCombine "MCS●t MCS●h" as "MCS_auth".
+          iMod ("Hclose" with "MCS") as "HΦ".            
+                      
+            
+            
+          iModIntro.
+          iSplitR "HΦ node_r HnP_t HnP_C HnP_frac".
+          { iNext. iExists (T+1), (H1 ∪ {[(k, T)]}), I1, J1, R1.
+            iFrame "∗%".   
+            rewrite (big_sepS_delete _ (domm I1) r); last by eauto.
+            iSplitL "Hl_r Hlif_r HnS_cl HnS_star Hφ HnS_frac HnS_oc HnS_si".
+            { iExists true, Cr', Br'. iFrame.
+            unfold nodeShared. iExists es, Ir, Jr, Rr.
+            iFrame "∗#".
+            iEval (rewrite <-beq_nat_refl). iFrame "%∗". }        
+          iApply (big_sepS_mono (λ y, ∃ (bn0 : bool) (Cn0 Bn0 : gmap K natUR),
+                                    lockLoc y ↦ #bn0
+                                  ∗ (if bn0 then True else
+                                     nodePred γ_e γ_c γ_b γ_t γ_s r y Cn0 Bn0)
+                                  ∗ nodeShared γ_I γ_J γ_R γ_e γ_c γ_b γ_f γ_cir
+                                            r y Cn0 Bn0 T H1 )%I
+                                 (λ y, ∃ (bn0 : bool) (Cn0 Bn0 : gmap K natUR),
+                                    lockLoc y ↦ #bn0
+                                  ∗ (if bn0 then True else
+                                     nodePred γ_e γ_c γ_b γ_t γ_s r y Cn0 Bn0)
+                                  ∗ nodeShared γ_I γ_J γ_R γ_e γ_c γ_b γ_f γ_cir
+                                            r y Cn0 Bn0 (T+1) (H1 ∪ {[(k, T)]}) )%I
+                                 (domm I1 ∖ {[r]})); try done.
+            intros y y_dom. assert (y ≠ r) as Hy by set_solver. iFrame. 
+            iIntros "Hstar"; iDestruct "Hstar" as (b C B)"(Hl & Hlif & HnS)".
+            iExists b, C, B; iFrame. 
+            iDestruct "HnS" as (esy Iy Jy Ry)"(HnS_frac & HnS_si & HnS_FP 
+                          & HnS_cl & HnS_oc & HnS_if & HnS_star & Hφ0 & Hφ)";
+            iExists esy, Iy, Jy, Ry; iFrame. 
             assert (y =? r = false) as Hyr by (rewrite beq_nat_false_iff; done);
-            iEval (rewrite Hyr); done. } 
+            iEval (rewrite Hyr).
+            iDestruct "Hφ0" as %Hφ0.
+            iPureIntro; split; try done.
+            intros k'. pose proof Hφ0 k' as Hφ0.
+            apply (Nat.le_trans _ T _); try done. lia. } 
           wp_pures.  
-          awp_apply (unlockNode_spec_high with "[] [] [HnP_t HnP_C HnP_frac node_n]")
+          awp_apply (unlockNode_spec_high with "[] [] [HnP_t HnP_C HnP_frac node_r]")
                 without "HΦ"; try done. iExists es, (T + 1). iFrame.
                 by iEval (rewrite <-beq_nat_refl).
           iAaccIntro with ""; try eauto with iFrame.
-                    
-  Admitted.
+  Qed.
 
 End multicopy.             
                     
